format-version: 1.2
data-version: releases/2026-01-16
idspace: dc http://purl.org/dc/elements/1.1/ 
idspace: oboInOwl http://www.geneontology.org/formats/oboInOwl# 
ontology: uo
property_value: owl:versionInfo "2026-01-16" xsd:string

[Term]
id: UO:0000000
name: unit
def: "A unit of measurement is a standardized quantity of a physical quality." [Wikipedia:Wikipedia]

[Term]
id: UO:0000001
name: length unit
def: "A unit which is a standard measure of the distance between two points." [Wikipedia:Wikipedia]
is_a: UO:0000000 ! unit

[Term]
id: UO:0000002
name: mass unit
def: "A unit which is a standard measure of the amount of matter/energy of a physical object." [Wikipedia:Wikipedia]
is_a: UO:0000000 ! unit

[Term]
id: UO:0000003
name: time unit
def: "A unit which is a standard measure of the dimension in which events occur in sequence." [Wikipedia:Wikipedia]
synonym: "time derived unit" EXACT []
is_a: UO:0000000 ! unit

[Term]
id: UO:0000004
name: electric current unit
def: "A unit which is a standard measure of the flow of electric charge." [Wikipedia:Wikipedia]
is_a: UO:0000000 ! unit

[Term]
id: UO:0000005
name: temperature unit
def: "A unit which is a standard measure of the average kinetic energy of the particles in a sample of matter." [Wikipedia:Wikipedia]
synonym: "temperature derived unit" EXACT []
is_a: UO:0000000 ! unit

[Term]
id: UO:0000006
name: substance unit
def: "A unit which is a standardised quantity of an element or compound with uniform composition." [Wikipedia:Wikipedia]
is_a: UO:0000000 ! unit

[Term]
id: UO:0000007
name: luminous intensity unit
def: "A unit which is a standard measure of the wavelength-weighted power emitted by a light source in a particular direction." [Wikipedia:Wikipedia]
is_a: UO:0000157 ! light unit

[Term]
id: UO:0000008
name: meter
def: "A length unit which is equal to the length of the path traveled by light in vacuum during a time interval of 1/299 792 458 of a second." [BIPM:BIPM, NIST:NIST]
synonym: "m" EXACT []
synonym: "metre" EXACT []
is_a: UO:0000045 ! base unit
is_a: UO:1000008 ! meter based unit

[Term]
id: UO:0000009
name: kilogram
def: "A mass unit which is equal to the mass of the International Prototype Kilogram kept by the BIPM at Svres, France." [BIPM:BIPM, NIST:NIST]
synonym: "kg" EXACT []
is_a: UO:0000045 ! base unit
is_a: UO:1000021 ! gram based unit
intersection_of: UO:1000021 ! gram based unit
intersection_of: has:prefix UO:0000294 ! kilo
relationship: has:prefix UO:0000294 ! kilo

[Term]
id: UO:0000010
name: second
def: "A time unit which is equal to the duration of 9 192 631 770 periods of the radiation corresponding to the transition between the two hyperfine levels of the ground state of the caesium 133 atom." [BIPM:BIPM, NIST:NIST]
synonym: "s" EXACT []
is_a: UO:0000045 ! base unit
is_a: UO:1000010 ! second based unit

[Term]
id: UO:0000011
name: ampere
def: "An electric current unit which is equal to the constant current which, if maintained in two straight parallel conductors of infinite length, of negligible circular cross-section, and placed 1 m apart in vacuum, would produce between these conductors a force equal to 2 x 10^[-7] newton per meter of length." [BIPM:BIPM, NIST:NIST]
synonym: "A" EXACT []
is_a: UO:0000045 ! base unit
is_a: UO:1000011 ! ampere based unit

[Term]
id: UO:0000012
name: kelvin
def: "A thermodynamic temperature unit which is equal to the fraction 1/273.16 of the thermodynamic temperature of the triple point of water." [BIPM:BIPM, NIST:NIST]
synonym: "K" EXACT []
is_a: UO:0000045 ! base unit
is_a: UO:1000012 ! kelvin based unit

[Term]
id: UO:0000013
name: mole
def: "A substance unit which is equal to the amount of substance of a molecular system which contains as many elementary entities as there are atoms in 0.012 kilogram of carbon 12." [BIPM:BIPM, NIST:NIST]
synonym: "mol" EXACT []
is_a: UO:0000045 ! base unit
is_a: UO:1000013 ! mole based unit

[Term]
id: UO:0000014
name: candela
def: "A luminous intensity unit which equal to the luminous intensity, in a given direction, of a source that emits monochromatic radiation of frequency 540 x 1012 hertz and that has a radiant intensity in that direction of 1/683 watt per steradian." [BIPM:BIPM, NIST:NIST]
synonym: "cd" EXACT []
is_a: UO:0000045 ! base unit
is_a: UO:1000014 ! candela based unit

[Term]
id: UO:0000015
name: centimeter
def: "A length unit which is equal to one hundredth of a meter or 10^[-2] m." [NIST:NIST]
synonym: "centimetre" EXACT []
synonym: "cm" EXACT []
is_a: UO:1000008 ! meter based unit
intersection_of: UO:1000008 ! meter based unit
intersection_of: has:prefix UO:0000298 ! centi
relationship: has:prefix UO:0000298 ! centi

[Term]
id: UO:0000016
name: millimeter
def: "A length unit which is equal to one thousandth of a meter or 10^[-3] m." [NIST:NIST]
synonym: "millimetre" EXACT []
synonym: "mm" EXACT []
is_a: UO:1000008 ! meter based unit
intersection_of: UO:1000008 ! meter based unit
intersection_of: has:prefix UO:0000297 ! milli
relationship: has:prefix UO:0000297 ! milli

[Term]
id: UO:0000017
name: micrometer
def: "A length unit which is equal to one millionth of a meter or 10^[-6] m." [NIST:NIST]
synonym: "micrometre" EXACT []
synonym: "micron" EXACT []
synonym: "um" EXACT []
is_a: UO:1000008 ! meter based unit
intersection_of: UO:1000008 ! meter based unit
intersection_of: has:prefix UO:0000299 ! micro
relationship: has:prefix UO:0000299 ! micro

[Term]
id: UO:0000018
name: nanometer
def: "A length unit which is equal to one thousandth of one millionth of a meter or 10^[-9] m." [NIST:NIST]
synonym: "nanometre" EXACT []
synonym: "nm" EXACT []
is_a: UO:1000008 ! meter based unit
intersection_of: UO:1000008 ! meter based unit
intersection_of: has:prefix UO:0000300 ! nano
relationship: has:prefix UO:0000300 ! nano

[Term]
id: UO:0000019
name: angstrom
def: "A length unit which is equal to 10 [-10] m." [NIST:NIST]
synonym: "Ã…" EXACT []
is_a: UO:1000019 ! angstrom based unit

[Term]
id: UO:0000020
name: picometer
def: "A length unit which is equal to 10^[-12] m." [NIST:NIST]
synonym: "picometre" EXACT []
synonym: "pm" EXACT []
is_a: UO:1000008 ! meter based unit
intersection_of: UO:1000008 ! meter based unit
intersection_of: has:prefix UO:0000302 ! pico
relationship: has:prefix UO:0000302 ! pico

[Term]
id: UO:0000021
name: gram
def: "A mass unit which is equal to one thousandth of a kilogram or 10^[-3] kg." [NIST:NIST]
synonym: "g" EXACT []
is_a: UO:1000021 ! gram based unit

[Term]
id: UO:0000022
name: milligram
def: "A mass unit which is equal to one thousandth of a gram or 10^[-3] g." [UOC:GVG]
synonym: "mg" EXACT []
is_a: UO:1000021 ! gram based unit
intersection_of: UO:1000021 ! gram based unit
intersection_of: has:prefix UO:0000297 ! milli
relationship: has:prefix UO:0000297 ! milli

[Term]
id: UO:0000023
name: microgram
def: "A mass unit which is equal to one millionth of a gram or 10^[-6] g." [UOC:GVG]
synonym: "ug" EXACT []
is_a: UO:1000021 ! gram based unit
intersection_of: UO:1000021 ! gram based unit
intersection_of: has:prefix UO:0000299 ! micro
relationship: has:prefix UO:0000299 ! micro

[Term]
id: UO:0000024
name: nanogram
def: "A mass unit which is equal to one thousandth of one millionth of a gram or 10^[-9] g." [UOC:GVG]
synonym: "ng" EXACT []
is_a: UO:1000021 ! gram based unit
intersection_of: UO:1000021 ! gram based unit
intersection_of: has:prefix UO:0000300 ! nano
relationship: has:prefix UO:0000300 ! nano

[Term]
id: UO:0000025
name: picogram
def: "A mass unit which is equal to 10^[-12] g." [UOC:GVG]
synonym: "pg" EXACT []
is_a: UO:1000021 ! gram based unit
intersection_of: UO:1000021 ! gram based unit
intersection_of: has:prefix UO:0000302 ! pico
relationship: has:prefix UO:0000302 ! pico

[Term]
id: UO:0000026
name: femtogram
def: "A mass unit which is equal to 10^[-15] g." [NIST:NIST]
synonym: "fg" EXACT []
is_a: UO:1000021 ! gram based unit
intersection_of: UO:1000021 ! gram based unit
intersection_of: has:prefix UO:0000303 ! femto
relationship: has:prefix UO:0000303 ! femto

[Term]
id: UO:0000027
name: degree Celsius
def: "A temperature unit which is equal to one kelvin degree. However, they have their zeros at different points. The centigrade scale has its zero at 273.15 K." [NIST:NIST]
synonym: "C" EXACT []
is_a: UO:1000027 ! degree Celsius based unit

[Term]
id: UO:0000028
name: millisecond
def: "A time unit which is equal to one thousandth of a second or 10^[-3] s." [NIST:NIST]
synonym: "ms" EXACT []
is_a: UO:1000010 ! second based unit
intersection_of: UO:1000010 ! second based unit
intersection_of: has:prefix UO:0000297 ! milli
relationship: has:prefix UO:0000297 ! milli

[Term]
id: UO:0000029
name: microsecond
def: "A time unit which is equal to one millionth of a second or 10^[-6] s." [NIST:NIST]
synonym: "us" EXACT []
is_a: UO:1000010 ! second based unit
intersection_of: UO:1000010 ! second based unit
intersection_of: has:prefix UO:0000299 ! micro
relationship: has:prefix UO:0000299 ! micro

[Term]
id: UO:0000030
name: picosecond
def: "A time unit which is equal to 10^[-12] s." [NIST:NIST]
synonym: "ps" EXACT []
is_a: UO:1000010 ! second based unit
intersection_of: UO:1000010 ! second based unit
intersection_of: has:prefix UO:0000302 ! pico
relationship: has:prefix UO:0000302 ! pico

[Term]
id: UO:0000031
name: minute
def: "A time unit which is equal to 60 seconds." [Wikipedia:Wikipedia]
synonym: "min" EXACT []
is_a: UO:1000031 ! minute based unit

[Term]
id: UO:0000032
name: hour
def: "A time unit which is equal to 3600 seconds or 60 minutes." [Wikipedia:Wikipedia]
synonym: "h" EXACT []
is_a: UO:1000032 ! hour based unit

[Term]
id: UO:0000033
name: day
def: "A time unit which is equal to 24 hours." [Wikipedia:Wikipedia]
is_a: UO:1000033 ! day based unit

[Term]
id: UO:0000034
name: week
def: "A time unit which is equal to 7 days." [Wikipedia:Wikipedia]
is_a: UO:1000034 ! week based unit

[Term]
id: UO:0000035
name: month
def: "A time unit which is approximately equal to the length of time of one of cycle of the moon's phases which in science is taken to be equal to 30 days." [Wikipedia:Wikipedia]
is_a: UO:1000035 ! month based unit

[Term]
id: UO:0000036
name: year
def: "A time unit which is equal to 12 months which in science is taken to be equal to 365.25 days." [Wikipedia:Wikipedia]
is_a: UO:1000036 ! year based unit

[Term]
id: UO:0000037
name: milliampere
def: "An electric current unit current which is equal to one thousandth of an ampere or 10^[-3] A." [UOC:GVG]
synonym: "mA" EXACT []
is_a: UO:1000011 ! ampere based unit
intersection_of: UO:1000011 ! ampere based unit
intersection_of: has:prefix UO:0000297 ! milli
relationship: has:prefix UO:0000297 ! milli

[Term]
id: UO:0000038
name: microampere
def: "An electric current unit current which is equal to one millionth of an ampere or 10^[-6] A." [UOC:GVG]
synonym: "uA" EXACT []
is_a: UO:1000011 ! ampere based unit
intersection_of: UO:1000011 ! ampere based unit
intersection_of: has:prefix UO:0000299 ! micro
relationship: has:prefix UO:0000299 ! micro

[Term]
id: UO:0000039
name: micromole
def: "A substance unit equal to a millionth of a mol or 10^[-6] mol." [NIST:NIST]
synonym: "umol" EXACT []
is_a: UO:1000013 ! mole based unit
intersection_of: UO:1000013 ! mole based unit
intersection_of: has:prefix UO:0000299 ! micro
relationship: has:prefix UO:0000299 ! micro

[Term]
id: UO:0000040
name: millimole
def: "A substance unit equal to a thousandth of a mol or 10^[-3] mol." [NIST:NIST]
synonym: "mmol" EXACT []
is_a: UO:1000013 ! mole based unit
intersection_of: UO:1000013 ! mole based unit
intersection_of: has:prefix UO:0000297 ! milli
relationship: has:prefix UO:0000297 ! milli

[Term]
id: UO:0000041
name: nanomole
def: "A substance unit equal to one thousandth of one millionth of a mole or 10^[-9] mol." [NIST:NIST]
synonym: "nmol" EXACT []
is_a: UO:1000013 ! mole based unit
intersection_of: UO:1000013 ! mole based unit
intersection_of: has:prefix UO:0000300 ! nano
relationship: has:prefix UO:0000300 ! nano

[Term]
id: UO:0000042
name: picomole
def: "A substance unit equal to 10^[-12] mol." [NIST:NIST]
synonym: "pmol" EXACT []
is_a: UO:1000013 ! mole based unit
intersection_of: UO:1000013 ! mole based unit
intersection_of: has:prefix UO:0000302 ! pico
relationship: has:prefix UO:0000302 ! pico

[Term]
id: UO:0000043
name: femtomole
def: "A substance unit equal to 10^[-15] mol." [NIST:NIST]
synonym: "fmol" EXACT []
is_a: UO:1000013 ! mole based unit
intersection_of: UO:1000013 ! mole based unit
intersection_of: has:prefix UO:0000303 ! femto
relationship: has:prefix UO:0000303 ! femto

[Term]
id: UO:0000044
name: attomole
def: "A substance unit equal to 10^[-18] mol." [NIST:NIST]
synonym: "amol" EXACT []
is_a: UO:1000013 ! mole based unit
intersection_of: UO:1000013 ! mole based unit
intersection_of: has:prefix UO:0000304 ! atto
relationship: has:prefix UO:0000304 ! atto

[Term]
id: UO:0000045
name: base unit
def: "A unit which is one of a particular measure to which all measures of that type can be related." [NIST:NIST]
is_a: UO:0000000 ! unit

[Term]
id: UO:0000046
name: prefix

[Term]
id: UO:0000047
name: area unit
def: "A unit which is a standard measure of the amount of a 2-dimensional flat surface." [UOC:GVG]
is_a: UO:0000000 ! unit

[Term]
id: UO:0000048
name: acceleration unit
def: "A unit which is a standard measure of the rate of change of velocity in either speed or direction." [Wikipedia:Wikipedia]
is_a: UO:0000000 ! unit

[Term]
id: UO:0000049
name: angular velocity unit
def: "A unit which is a standard measure of the rate of angular movement about an axis; the angle rotated in a given time." [Wikipedia:Wikipedia]
is_a: UO:0000000 ! unit

[Term]
id: UO:0000050
name: angular acceleration unit
def: "A unit which is a standard measure of the rate of change of angular velocity." [Wikipedia:Wikipedia]
is_a: UO:0000000 ! unit

[Term]
id: UO:0000051
name: concentration unit
def: "A unit which represents a standard measurement of how much of a given substance there is mixed with another substance." [UOC:GVG]
is_a: UO:0000000 ! unit

[Term]
id: UO:0000052
name: mass density unit
def: "A density unit which is a standard measure of the mass of a substance in a given volume." [UOC:GVG]
synonym: "mass per unit volume" EXACT []
is_a: UO:0000182 ! density unit

[Term]
id: UO:0000053
name: luminance unit
def: "A unit which is a standard measure of the luminous intensity impinging on a given area." [Wikipedia:Wikipedia]
is_a: UO:0000157 ! light unit

[Term]
id: UO:0000054
name: area density unit
def: "A density unit which is a standard measure of the mass exerting an influence on a given area." [Wikipedia:Wikipedia]
synonym: "mass per unit area unit" EXACT []
is_a: UO:0000182 ! density unit

[Term]
id: UO:0000055
name: molar mass unit
def: "A unit which is a standard measure of the mass of a homogeneous substance containing 6.02 x 1023 atoms or molecules." [Wikipedia:Wikipedia]
is_a: UO:0000002 ! mass unit

[Term]
id: UO:0000056
name: molar volume unit
def: "A unit which is a standard measure of the volume of a homogeneous substance containing 6.02 x 1023 atoms or molecules." [Wikipedia:Wikipedia]
is_a: UO:0000095 ! volume unit

[Term]
id: UO:0000057
name: momentum unit
def: "A unit which is a standard measure of the quantity of motion measured by the product of mass and velocity." [Wikipedia:Wikipedia]
is_a: UO:0000000 ! unit

[Term]
id: UO:0000058
name: rotational frequency unit
def: "A unit which is a standard measure of the number of rotations in a given time." [NIST:NIST]
is_a: UO:0000105 ! frequency unit

[Term]
id: UO:0000059
name: specific volume unit
def: "A unit which is a standard measure of the volume of a given mass of substance (the reciprocal of density)." [Wikipedia:Wikipedia]
is_a: UO:0000095 ! volume unit

[Term]
id: UO:0000060
name: speed/velocity unit
def: "A unit which is a standard measure of the rate of movement. Speed is measured in the same physical units of measurement as velocity, but does not contain the element of direction that velocity has. Speed is thus the magnitude component of velocity." [Wikipedia:Wikipedia]
is_a: UO:0000000 ! unit

[Term]
id: UO:0000061
name: unit of molarity
def: "A concentration unit which is a standard measure of the number of moles of a given substance per liter of solution." [UOC:GVG]
is_a: UO:0000051 ! concentration unit

[Term]
id: UO:0000062
name: molar
def: "A unit of concentration which expresses a concentration of 1 mole of solute per liter of solution (mol/L)." [UOC:GVG]
synonym: "M" EXACT []
is_a: UO:1000062 ! molar based unit

[Term]
id: UO:0000063
name: millimolar
def: "A unit of molarity which is equal to one thousandth of a molar or 10^[-3] M." [UOC:GVG]
synonym: "mM" EXACT []
is_a: UO:1000062 ! molar based unit
intersection_of: UO:1000062 ! molar based unit
intersection_of: has:prefix UO:0000297 ! milli
relationship: has:prefix UO:0000297 ! milli

[Term]
id: UO:0000064
name: micromolar
def: "A unit of molarity which is equal to one millionth of a molar or 10^[-6] M." [UOC:GVG]
synonym: "uM" EXACT []
is_a: UO:1000062 ! molar based unit
intersection_of: UO:1000062 ! molar based unit
intersection_of: has:prefix UO:0000299 ! micro
relationship: has:prefix UO:0000299 ! micro

[Term]
id: UO:0000065
name: nanomolar
def: "A unit of molarity which is equal to one thousandth of one millionth of a molar or 10^[-9] M." [UOC:GVG]
synonym: "nM" EXACT []
is_a: UO:1000062 ! molar based unit
intersection_of: UO:1000062 ! molar based unit
intersection_of: has:prefix UO:0000300 ! nano
relationship: has:prefix UO:0000300 ! nano

[Term]
id: UO:0000066
name: picomolar
def: "A unit of molarity which is equal to 10^[-12] M." [UOC:GVG]
synonym: "pM" EXACT []
is_a: UO:1000062 ! molar based unit
intersection_of: UO:1000062 ! molar based unit
intersection_of: has:prefix UO:0000302 ! pico
relationship: has:prefix UO:0000302 ! pico

[Term]
id: UO:0000067
name: unit of molality
def: "A concentration unit which is a standard measure of the number of moles of a given substance per kilogram of solvent." [UOC:GVG]
is_a: UO:0000051 ! concentration unit

[Term]
id: UO:0000068
name: molal
def: "A unit of concentration which expresses a concentration of a solution of 1 mole per kilogram of solvent (mol/kg)." [UOC:GVG]
synonym: "m" EXACT []
is_a: UO:1000068 ! molal based unit

[Term]
id: UO:0000069
name: millimolal
def: "A molality unit which is equal to one thousandth of a molal or 10^[-3] m." [UOC:GVG]
synonym: "mm" EXACT []
is_a: UO:1000068 ! molal based unit
intersection_of: UO:1000068 ! molal based unit
intersection_of: has:prefix UO:0000297 ! milli
relationship: has:prefix UO:0000297 ! milli

[Term]
id: UO:0000070
name: micromolal
def: "A molality unit which is equal to one millionth of a molal or 10^[-6] m." [UOC:GVG]
synonym: "um" EXACT []
is_a: UO:1000068 ! molal based unit
intersection_of: UO:1000068 ! molal based unit
intersection_of: has:prefix UO:0000299 ! micro
relationship: has:prefix UO:0000299 ! micro

[Term]
id: UO:0000071
name: nanomolal
def: "A molality unit which is equal to one thousandth of one millionth of a molal or 10^[-9] m." [UOC:GVG]
synonym: "nm" EXACT []
is_a: UO:1000068 ! molal based unit
intersection_of: UO:1000068 ! molal based unit
intersection_of: has:prefix UO:0000300 ! nano
relationship: has:prefix UO:0000300 ! nano

[Term]
id: UO:0000072
name: picomolal
def: "A molality unit which is equal to 10^[-12] m." [UOC:GVG]
synonym: "pm" EXACT []
is_a: UO:1000068 ! molal based unit
intersection_of: UO:1000068 ! molal based unit
intersection_of: has:prefix UO:0000302 ! pico
relationship: has:prefix UO:0000302 ! pico

[Term]
id: UO:0000073
name: femtomolar
def: "A unit of molarity which is equal to 10^[-15] M." [UOC:GVG]
synonym: "fM" EXACT []
is_a: UO:1000062 ! molar based unit
intersection_of: UO:1000062 ! molar based unit
intersection_of: has:prefix UO:0000303 ! femto
relationship: has:prefix UO:0000303 ! femto

[Term]
id: UO:0000074
name: unit of normality
def: "A unit of concentration which highlights the chemical nature of salts." [Wikipedia:Wikipedia]
is_a: UO:0000051 ! concentration unit

[Term]
id: UO:0000075
name: normal
def: "A unit of concentration which is one gram equivalent of a solute per liter of solution. A gram equivalent weight or equivalent is a measure of the reactive capacity of a given molecule." [Wikipedia:Wikipedia]
synonym: "N" EXACT []
is_a: UO:1000075 ! normal based unit

[Term]
id: UO:0000076
name: mole fraction
def: "A concentration unit which denotes the number of moles of solute as a proportion of the total number of moles in a solution." [Wikipedia:Wikipedia]
synonym: "(x)" EXACT []
synonym: "chi" EXACT []
is_a: UO:1000076 ! mole fraction based unit

[Term]
id: UO:0000077
name: meter per second per second
def: "An acceleration unit which is equal to the acceleration an object changing its velocity by 1meter/s over a time period that equals one second." [NIST:NIST]
synonym: "m/s^[2]" EXACT []
synonym: "metre per second per second" EXACT []
is_a: UO:1000077 ! meter per second per second based unit

[Term]
id: UO:0000078
name: radian per second per second
def: "An angular unit acceleration which is equal to the angular acceleration of an object changing its angular velocity by 1rad/s over a time period that equals one second." [NIST:NIST]
synonym: "alpha" EXACT []
synonym: "rad/s^[2]" EXACT []
is_a: UO:1000078 ! radian per second per second based unit

[Term]
id: UO:0000079
name: radian per second
def: "An angular unit velocity which is equal to about 9.54930 rpm (revolutions per minute)." [NIST:NIST]
synonym: "rad/s" EXACT []
is_a: UO:1000079 ! radian per second based unit

[Term]
id: UO:0000080
name: square meter
def: "An area unit which is equal to an area enclosed by a square with sides each 1 meter long." [NIST:NIST]
synonym: "m^[2]" EXACT []
synonym: "square metre" EXACT []
is_a: UO:1000080 ! square meter based unit

[Term]
id: UO:0000081
name: square centimeter
def: "An area unit which is equal to one ten thousandth of a square meter or 10^[-4] m^[2]." [NIST:NIST]
synonym: "cm^[2]" EXACT []
synonym: "square centimetre" EXACT []
is_a: UO:1000081 ! square centimeter based unit

[Term]
id: UO:0000082
name: square millimeter
def: "An area unit which is equal to one millionth of a square meter or 10^[-6] m^[2]." [NIST:NIST]
synonym: "mm^[2]" EXACT []
synonym: "square millimetre" EXACT []
is_a: UO:1000082 ! square millimeter based unit

[Term]
id: UO:0000083
name: kilogram per cubic meter
def: "A mass unit density which is equal to mass of an object in kilograms divided by the volume in cubic meters." [UOC:GVG]
synonym: "kg/m^[3]" EXACT []
synonym: "kilogram per cubic metre" EXACT []
is_a: UO:0000052 ! mass density unit

[Term]
id: UO:0000084
name: gram per cubic centimeter
def: "A mass unit density which is equal to mass of an object in grams divided by the volume in cubic centimeters." [UOC:GVG]
synonym: "g/cm^[3]" EXACT []
synonym: "gram per cubic centimetre" EXACT []
is_a: UO:1000084 ! gram per cubic centimeter based unit

[Term]
id: UO:0000085
name: candela per square meter
def: "A luminance unit which is equal to a luminous intensity of one candela radiating from a surface whose area is one square meter." [NIST:NIST]
synonym: "candela per square metre" EXACT []
synonym: "cd/m^[2]" EXACT []
is_a: UO:1000085 ! candela per square meter based unit

[Term]
id: UO:0000086
name: kilogram per square meter
def: "An area density unit which is equal to the mass of an object in kilograms divided by the surface area in meters squared." [NIST:NIST]
synonym: "kg/m^[2]" EXACT []
synonym: "kilogram per square metre" EXACT []
is_a: UO:1010049 ! gram per square meter based unit
intersection_of: UO:1010049 ! gram per square meter based unit
intersection_of: has:prefix UO:0000294 ! kilo
relationship: has:prefix UO:0000294 ! kilo

[Term]
id: UO:0000087
name: kilogram per mole
def: "A molar mass unit which is equal to one kilogram of mass of one mole of chemical element or chemical compound." [NIST:NIST]
synonym: "kg/mol" EXACT []
is_a: UO:1000088 ! gram per mole based unit
intersection_of: UO:1000088 ! gram per mole based unit
intersection_of: has:prefix UO:0000294 ! kilo
relationship: has:prefix UO:0000294 ! kilo

[Term]
id: UO:0000088
name: gram per mole
def: "A molar mass unit which is equal to one gram of mass of one mole of chemical element or chemical compound." [NIST:NIST]
synonym: "g/mol" EXACT []
is_a: UO:1000088 ! gram per mole based unit

[Term]
id: UO:0000089
name: cubic meter per mole
def: "A molar volume unit which is equal to 1 cubic meter occupied by one mole of a substance in the form of a solid, liquid, or gas." [NIST:NIST]
synonym: "cubic metre per mole" EXACT []
synonym: "m^[3]/mol" EXACT []
is_a: UO:1000089 ! cubic meter per mole based unit

[Term]
id: UO:0000090
name: cubic centimeter per mole
def: "A molar volume unit which is equal to 1 cubic centimeter occupied by one mole of a substance in the form of a solid, liquid, or gas." [NIST:NIST]
synonym: "cm^[3]/mol" EXACT []
synonym: "cubic centimetre per mole" EXACT []
is_a: UO:1000090 ! cubic centimeter per mole based unit

[Term]
id: UO:0000091
name: kilogram meter per second
def: "A momentum unit which is equal to the momentum of a one kilogram mass object with a speed of one meter per second." [NIST:NIST]
synonym: "kg.m/s" EXACT []
synonym: "kilogram metre per second" EXACT []
is_a: UO:0000057 ! momentum unit

[Term]
id: UO:0000092
name: turns per second
def: "A rotational frequency unit which is equal to the number complete turn in a period of time that equals to 1 second." [NIST:NIST]
synonym: "1/s" EXACT []
synonym: "one turn per second" EXACT []
is_a: UO:1000092 ! turns per second based unit

[Term]
id: UO:0000093
name: cubic meter per kilogram
def: "A specific volume unit which is equal to one cubic meter volume occupied by one kilogram of a particular substance." [NIST:NIST]
synonym: "cubic metre per kilogram" EXACT []
synonym: "m^[3]/kg" EXACT []
is_a: UO:1000093 ! cubic meter per kilogram based unit

[Term]
id: UO:0000094
name: meter per second
def: "A speed/velocity unit which is equal to the speed of an object traveling 1 meter distance in one second." [NIST:NIST]
synonym: "m/s" EXACT []
synonym: "metre per second" EXACT []
is_a: UO:1000094 ! meter per second based unit

[Term]
id: UO:0000095
name: volume unit
def: "A unit which is a standard measure of the amount of space occupied by any substance, whether solid, liquid, or gas." [NIST:NIST]
is_a: UO:0000000 ! unit

[Term]
id: UO:0000096
name: cubic meter
def: "A volume unit which is equal to the volume of a cube with edges one meter in length. One cubic meter equals to 1000 liters." [NIST:NIST]
synonym: "cubic metre" EXACT []
synonym: "m^[3]" EXACT []
is_a: UO:1000096 ! cubic meter based unit

[Term]
id: UO:0000097
name: cubic centimeter
def: "A volume unit which is equal to one millionth of a cubic meter or 10^[-9] m^[3], or to 1 ml." [NIST:NIST]
synonym: "cc" EXACT []
synonym: "cm^3" EXACT []
synonym: "cubic centimetre" EXACT []
is_a: UO:1000097 ! cubic centimeter based unit

[Term]
id: UO:0000098
name: milliliter
def: "A volume unit which is equal to one thousandth of a liter or 10^[-3] L, or to 1 cubic centimeter." [NIST:NIST]
synonym: "millilitre" EXACT []
synonym: "ml" EXACT []
is_a: UO:1000099 ! liter based unit
intersection_of: UO:1000099 ! liter based unit
intersection_of: has:prefix UO:0000297 ! milli
relationship: has:prefix UO:0000297 ! milli

[Term]
id: UO:0000099
name: liter
def: "A volume unit which is equal to one thousandth of a cubic meter or 10^[-3] m^[3], or to 1 decimeter." [NIST:NIST]
synonym: "L" EXACT []
synonym: "l" EXACT []
synonym: "litre" EXACT []
is_a: UO:1000099 ! liter based unit

[Term]
id: UO:0000100
name: cubic decimeter
def: "A volume unit which is equal to one thousand of a cubic meter or 10^[-3] m^[3], or to 1 L." [NIST:NIST]
synonym: "cubic decimetre" EXACT []
synonym: "dm^[3]" EXACT []
is_a: UO:1000100 ! cubic decimeter based unit

[Term]
id: UO:0000101
name: microliter
def: "A volume unit which is equal to one millionth of a liter or 10^[-6] L." [NIST:NIST]
synonym: "microlitre" EXACT []
synonym: "ul" EXACT []
is_a: UO:1000099 ! liter based unit
intersection_of: UO:1000099 ! liter based unit
intersection_of: has:prefix UO:0000299 ! micro
relationship: has:prefix UO:0000299 ! micro

[Term]
id: UO:0000102
name: nanoliter
def: "A volume unit which is equal to one thousandth of one millionth of a liter or 10^[-9] L." [NIST:NIST]
synonym: "nanolitre" EXACT []
synonym: "nl" EXACT []
is_a: UO:1000099 ! liter based unit
intersection_of: UO:1000099 ! liter based unit
intersection_of: has:prefix UO:0000300 ! nano
relationship: has:prefix UO:0000300 ! nano

[Term]
id: UO:0000103
name: picoliter
def: "A volume unit which is equal to 10^[-12] L." [NIST:NIST]
synonym: "picolitre" EXACT []
synonym: "pl" EXACT []
is_a: UO:1000099 ! liter based unit
intersection_of: UO:1000099 ! liter based unit
intersection_of: has:prefix UO:0000302 ! pico
relationship: has:prefix UO:0000302 ! pico

[Term]
id: UO:0000104
name: femtoliter
def: "A volume unit which is equal to 10^[-15] L." [NIST:NIST]
synonym: "femtolitre" EXACT []
synonym: "fl" EXACT []
is_a: UO:1000099 ! liter based unit
intersection_of: UO:1000099 ! liter based unit
intersection_of: has:prefix UO:0000303 ! femto
relationship: has:prefix UO:0000303 ! femto

[Term]
id: UO:0000105
name: frequency unit
def: "A unit which is a standard measure of the number of repetitive actions in a particular time." [NIST:NIST]
is_a: UO:0000000 ! unit

[Term]
id: UO:0000106
name: hertz
def: "A frequency unit which is equal to 1 complete cycle of a recurring phenomenon in 1 second." [NIST:NIST]
synonym: "Hz" EXACT []
synonym: "s^1" EXACT []
is_a: UO:1000106 ! hertz based unit

[Term]
id: UO:0000107
name: force unit
def: "A unit which is a standard measure of the force is applied when a mass is accelerated." [NIST:NIST]
is_a: UO:0000000 ! unit

[Term]
id: UO:0000108
name: newton
def: "A force unit which is equal to the force required to cause an acceleration of 1m/s2 of a mass of 1 Kg in the direction of the force." [NIST:NIST]
synonym: "N" EXACT []
is_a: UO:1000108 ! newton based unit

[Term]
id: UO:0000109
name: pressure unit
def: "A unit which is a standard measure of the force applied to a given area." [NIST:NIST]
is_a: UO:0000000 ! unit

[Term]
id: UO:0000110
name: pascal
def: "A pressure unit which is equal to the pressure or stress on a surface caused by a force of 1 newton spread over a surface of 1 m^[2]." [NIST:NIST]
synonym: "Pa" EXACT []
is_a: UO:1000110 ! pascal based unit

[Term]
id: UO:0000111
name: energy unit
def: "A unit which is a standard measure of the work done by a certain force (gravitational, electric, magnetic, force of inertia, etc)." [NIST:NIST]
is_a: UO:0000000 ! unit

[Term]
id: UO:0000112
name: joule
def: "An energy unit which is equal to the energy required when a force of 1 newton moves an object 1 meter in the direction of the force." [NIST:NIST]
synonym: "J" EXACT []
is_a: UO:1000112 ! joule based unit

[Term]
id: UO:0000113
name: power unit
def: "A unit which is a standard measure power or the rate of doing work." [NIST:NIST]
is_a: UO:0000000 ! unit

[Term]
id: UO:0000114
name: watt
def: "A power unit which is equal to the power used when work is done at the rate of 1 joule per second." [NIST:NIST]
synonym: "W" EXACT []
is_a: UO:1000114 ! watt based unit

[Term]
id: UO:0000115
name: illuminance unit
def: "A unit which is a standard measure of the luminous flux incident on a unit area." [Wikipedia:Wikipedia]
is_a: UO:0000157 ! light unit

[Term]
id: UO:0000116
name: lux
def: "An illuminance unit which is equal to the illuminance produced by 1 lumen evenly spread over an area 1 m^[2]." [NIST:NIST]
synonym: "lx" EXACT []
is_a: UO:1000116 ! lux based unit

[Term]
id: UO:0000117
name: luminous flux unit
def: "A unit which is a standard measure of the flow of radiant energy." [Wikipedia:Wikipedia]
is_a: UO:0000157 ! light unit

[Term]
id: UO:0000118
name: lumen
def: "A luminous flux unit which is equal to the luminous flux emitted into 1 steradian by a point source of 1 candela." [NIST:NIST]
synonym: "lm" EXACT []
is_a: UO:1000118 ! lumen based unit

[Term]
id: UO:0000119
name: catalytic activity unit
def: "A unit which is a standard measure of the amount of the action of a catalyst." [NIST:NIST]
is_a: UO:0000000 ! unit

[Term]
id: UO:0000120
name: katal
def: "A catalytic unit activity which is equal to the activity of a catalyst in moles per second, such as the amount of an enzyme needed to transform one mole of substrate per second." [NIST:NIST]
synonym: "kat" EXACT []
is_a: UO:1000120 ! katal based unit

[Term]
id: UO:0000121
name: angle unit
def: "A unit which is a standard measure of the figure or space formed by the junction of two lines or planes." [Wikipedia:Wikipedia]
is_a: UO:0000000 ! unit

[Term]
id: UO:0000122
name: plane angle unit
def: "A unit which is a standard measure of the angle formed by two straight lines in the same plane." [Wikipedia:Wikipedia]
is_a: UO:0000121 ! angle unit

[Term]
id: UO:0000123
name: radian
def: "A plane angle unit which is equal to the angle subtended at the center of a circle by an arc equal in length to the radius of the circle, approximately 57 degrees 17 minutes and 44.6 seconds." [NIST:NIST]
synonym: "rad" EXACT []
is_a: UO:1000123 ! radian based unit

[Term]
id: UO:0000124
name: solid angle unit
def: "A unit which is a standard measure of the angle formed by three or more planes intersecting at a common point." [Wikipedia:Wikipedia]
is_a: UO:0000121 ! angle unit

[Term]
id: UO:0000125
name: steradian
def: "A solid angle unit which is equal to the solid angle subtended at the center of a sphere by an area on the surface of the sphere that is equal to the radius squared." [NIST:NIST]
synonym: "sr" EXACT []
is_a: UO:1000125 ! steradian based unit

[Term]
id: UO:0000127
name: radiation unit
def: "A unit which is a standard measure of the amount of radiation emitted by a given radiation source as well as the amount of radiation absorbed or deposited in a specific material by a radiation source." [OCRBS:OCRBS]
is_a: UO:0000000 ! unit

[Term]
id: UO:0000128
name: activity (of a radionuclide) unit
def: "A unit which is a standard measure of the transformation (disintegration) rate of a radioactive substance." [DEFRA:DEFRA]
is_a: UO:0000127 ! radiation unit

[Term]
id: UO:0000129
name: absorbed dose unit
def: "A unit which is a standard measure of the energy imparted by ionizing radiation to unit mass of matter such as tissue." [DEFRA:DEFRA]
is_a: UO:0000127 ! radiation unit

[Term]
id: UO:0000130
name: dose equivalent unit
def: "A unit which is a standard measure of the expression of dose in terms of its biological effect." [ORCBS:ORCBS]
is_a: UO:0000127 ! radiation unit

[Term]
id: UO:0000131
name: exposure unit
def: "A unit which is a standard measure of the quantity that expresses the ability of radiation to ionize air and thereby create electric charges which can be collected and measured." [ORCBS:ORCBS]
is_a: UO:0000127 ! radiation unit

[Term]
id: UO:0000132
name: becquerel
def: "An activity (of a radionuclide) unit which is equal to the activity of a quantity of radioactive material in which one nucleus decays per second or there is one atom disintegration per second (dps)." [NIST:NIST]
synonym: "Bq" EXACT []
is_a: UO:1000132 ! becquerel based unit

[Term]
id: UO:0000133
name: curie
def: "An activity (of a radionuclide) unit which is equal to the activity of a quantity of radioactive material in which there are 3.7 x 10^[10] atom disintegration per second (dps)." [ORCBS:ORCBS]
synonym: "Ci" EXACT []
is_a: UO:1000133 ! curie based unit

[Term]
id: UO:0000134
name: gray
def: "An absorbed dose unit which is equal to the absorption of one joule of radiation energy by one kilogram of matter." [NIST:NIST]
synonym: "Gy" EXACT []
is_a: UO:1000134 ! gray based unit

[Term]
id: UO:0000135
name: rad
def: "An absorbed dose unit which is equal to 0.01 gray (Gy)." [Wikipedia:Wikipedia]
is_a: UO:1000135 ! rad based unit

[Term]
id: UO:0000136
name: roentgen
def: "An exposure unit which is equal to the amount of radiation required to liberate positive and negative charges of one electrostatic unit of charge in 1 cm^[3] of air at standard temperature and pressure (STP). This corresponds to the generation of approximately 2.0810^[9] ion pairs." [Wikipedia:Wikipedia]
synonym: "R" EXACT []
is_a: UO:1000136 ! roentgen based unit

[Term]
id: UO:0000137
name: sievert
def: "A dose equivalent unit which is equal to the absorption of one joule of radiation energy by one kilogram of matter." [NIST:NIST]
synonym: "Sv" EXACT []
is_a: UO:1000137 ! sievert based unit

[Term]
id: UO:0000138
name: millisievert
def: "A dose equivalent unit which is equal to one thousandth of a sievert or 10^[-3] Sv." [NIST:NIST]
synonym: "mSv" EXACT []
is_a: UO:1000137 ! sievert based unit
intersection_of: UO:1000137 ! sievert based unit
intersection_of: has:prefix UO:0000297 ! milli
relationship: has:prefix UO:0000297 ! milli

[Term]
id: UO:0000139
name: microsievert
def: "A dose equivalent unit which is equal to one millionth of a sievert or 10^[-6] Sv." [NIST:NIST]
synonym: "uSv" EXACT []
is_a: UO:1000137 ! sievert based unit
intersection_of: UO:1000137 ! sievert based unit
intersection_of: has:prefix UO:0000299 ! micro
relationship: has:prefix UO:0000299 ! micro

[Term]
id: UO:0000140
name: Roentgen equivalent man
def: "A dose equivalent unit which when multiplied by hundred is equal to one sievert or 1 Sv. 1 Sv is equal to 100 rem." [Wikipedia:Wikipedia]
synonym: "rem" EXACT []
is_a: UO:1000140 ! Roentgen equivalent man based unit

[Term]
id: UO:0000141
name: microgray
def: "An absorbed dose unit which is equal to one millionth of a gray or 10^[-6] Gy." [NIST:NIST]
synonym: "uGy" EXACT []
is_a: UO:1000134 ! gray based unit
intersection_of: UO:1000134 ! gray based unit
intersection_of: has:prefix UO:0000299 ! micro
relationship: has:prefix UO:0000299 ! micro

[Term]
id: UO:0000142
name: milligray
def: "An absorbed dose unit which is equal to one thousandth of a gray or 10^[-3] Gy." [NIST:NIST]
synonym: "mGy" EXACT []
is_a: UO:1000134 ! gray based unit
intersection_of: UO:1000134 ! gray based unit
intersection_of: has:prefix UO:0000297 ! milli
relationship: has:prefix UO:0000297 ! milli

[Term]
id: UO:0000143
name: nanogray
def: "An absorbed dose unit which is equal to one thousandth of a millionth of a gray or 10^[-9] Gy." [NIST:NIST]
synonym: "nGy" EXACT []
is_a: UO:1000134 ! gray based unit
intersection_of: UO:1000134 ! gray based unit
intersection_of: has:prefix UO:0000300 ! nano
relationship: has:prefix UO:0000300 ! nano

[Term]
id: UO:0000144
name: nanosievert
def: "A dose equivalent unit which is equal to one thousandth of a millionth of a sievert or 10^[-9] Sv." [NIST:NIST]
synonym: "nSv" EXACT []
is_a: UO:1000137 ! sievert based unit
intersection_of: UO:1000137 ! sievert based unit
intersection_of: has:prefix UO:0000300 ! nano
relationship: has:prefix UO:0000300 ! nano

[Term]
id: UO:0000145
name: millicurie
def: "An activity (of a radionuclide) unit which is equal to one thousandth of a curie or 10^[-3] Ci." [ORCBS:ORCBS]
synonym: "mCi" EXACT []
is_a: UO:1000133 ! curie based unit
intersection_of: UO:1000133 ! curie based unit
intersection_of: has:prefix UO:0000297 ! milli
relationship: has:prefix UO:0000297 ! milli

[Term]
id: UO:0000146
name: microcurie
def: "An activity (of a radionuclide) unit which is equal to one millionth of a curie or 10^[-6] Ci." [ORCBS:ORCBS]
synonym: "uCi" EXACT []
is_a: UO:1000133 ! curie based unit
intersection_of: UO:1000133 ! curie based unit
intersection_of: has:prefix UO:0000299 ! micro
relationship: has:prefix UO:0000299 ! micro

[Term]
id: UO:0000147
name: disintegrations per minute
def: "An activity (of a radionuclide) unit which is equal to the activity of a quantity of radioactive material in which one nucleus decays per minute or there is one atom disintegration per minute." [ORCBS:ORCBS]
synonym: "dpm" EXACT []
is_a: UO:1000147 ! disintegrations per minute based unit

[Term]
id: UO:0000148
name: counts per minute
def: "An activity (of a radionuclide) unit which is equal to the number of light emissions produced by ionizing radiation in one minute." [ORCBS:ORCBS]
synonym: "cpm" EXACT []
is_a: UO:1000148 ! counts per minute based unit

[Term]
id: UO:0000150
name: nanosecond
def: "A time unit which is equal to one thousandth of one millionth of a second or 10^[-9] s." [NIST:NIST]
synonym: "ns" EXACT []
is_a: UO:1000010 ! second based unit
intersection_of: UO:1000010 ! second based unit
intersection_of: has:prefix UO:0000300 ! nano
relationship: has:prefix UO:0000300 ! nano

[Term]
id: UO:0000151
name: century
def: "A time unit which is equal to 100 years." [Wikipedia:Wikipedia]
is_a: UO:1000151 ! century based unit

[Term]
id: UO:0000152
name: half life
def: "A time unit which represents the period over which the activity or concentration of a specified chemical or element falls to half its original activity or concentration." [MGED:MGED]
is_a: UO:1000152 ! half life based unit

[Term]
id: UO:0000153
name: foot candle
def: "An illuminance unit which is equal to the illuminance produced by 1 lumen evenly spread over an area 1 foot^[2]. One footcandle is equal to 10.76 lux." [Wikipedia:Wikipedia]
synonym: "ft-c" EXACT []
is_a: UO:1000153 ! foot candle based unit

[Term]
id: UO:0000154
name: irradiance unit
def: "A unit which is a standard measure of the power of electromagnetic radiation at a surface, per unit area." [Wikipedia:Wikipedia]
is_a: UO:0000157 ! light unit

[Term]
id: UO:0000155
name: watt per square meter
def: "An irradiance unit which is equal to 1 watt of radiant power incident per one square meter surface area." [NIST:NIST]
synonym: "W/m^[2]" EXACT []
synonym: "watt per square metre" EXACT []
is_a: UO:1000155 ! watt per square meter based unit

[Term]
id: UO:0000156
name: einstein per square meter per second
def: "An irradiance unit which is equal to one einstein per square meter per second. One einstein is one mole of photons, regardless of their frequency. Therefore, the number of photons in an einstein is Avogadro's number." [Wikipedia:Wikipedia]
synonym: "einstein per square metre per second" EXACT []
synonym: "einstein/sm^[2]" EXACT []
synonym: "mole per second and square meter mol/sm^2" EXACT []
is_a: UO:1000156 ! einstein per square meter per second based unit

[Term]
id: UO:0000157
name: light unit
def: "A unit which is a standard measure of the intensity of light." [NIST:NIST]
is_a: UO:0000000 ! unit

[Term]
id: UO:0000158
name: watt per steradian per square meter
def: "A radiance unit which is equal to one watt of radiant power incident per steradian solid angle per one square meter projected area of the source, as viewed from the given direction." [NIST:NIST]
synonym: "W/sr m^[2]" EXACT []
synonym: "watt per steradian per square metre" EXACT []
is_a: UO:1000158 ! watt per steradian per square meter based unit

[Term]
id: UO:0000159
name: radiant intensity unit
def: "A unit which is a standard measure of the intensity of electromagnetic radiation." [Wikipedia:Wikipedia]
is_a: UO:0000157 ! light unit

[Term]
id: UO:0000160
name: microeinstein per square meter per second
def: "An irradiance unit which is equal to one microeinstein per square meter per second or 10^[-6] microeinstein/sm^[2]." [Wikipedia:Wikipedia]
synonym: "microeinstein per square metre per second" EXACT []
synonym: "micromole per second and square meter mmol/sm^2" EXACT []
synonym: "umicroeinstein/sm^[2]" EXACT []
is_a: UO:1000156 ! einstein per square meter per second based unit
intersection_of: UO:1000156 ! einstein per square meter per second based unit
intersection_of: has:prefix UO:0000299 ! micro
relationship: has:prefix UO:0000299 ! micro

[Term]
id: UO:0000161
name: radiance unit
def: "A unit which is a standard measure of the power of electromagnetic radiation through space or through a material medium in the form of electromagnetic waves." [Wikipedia:Wikipedia]
is_a: UO:0000157 ! light unit

[Term]
id: UO:0000162
name: watt per steradian
def: "A radiant intensity unit which is equal to one kilogram meter squared per second cubed per steradian." [NIST:NIST]
synonym: "W/sr" EXACT []
is_a: UO:1000162 ! watt per steradian based unit

[Term]
id: UO:0000163
name: mass percentage
def: "A dimensionless concentration unit which denotes the mass of a substance in a mixture as a percentage of the mass of the entire mixture." [Wikipedia:Wikipedia]
synonym: "w/w" EXACT []
synonym: "weight-weight percentage" EXACT []
is_a: UO:1000163 ! mass percentage based unit

[Term]
id: UO:0000164
name: mass volume percentage
def: "A dimensionless concentration unit which denotes the mass of the substance in a mixture as a percentage of the volume of the entire mixture." [UOC:GVG]
synonym: "(w/v)" EXACT []
synonym: "weight-volume percentage" EXACT []
is_a: UO:1000164 ! mass volume percentage based unit

[Term]
id: UO:0000165
name: volume percentage
def: "A dimensionless concentration unit which denotes the volume of the solute in mL per 100 mL of the resulting solution." [UOC:GVG]
synonym: "% (v/v)" EXACT []
is_a: UO:1000165 ! volume percentage based unit

[Term]
id: UO:0000166
name: parts per notation unit
def: "A dimensionless concentration notation which describes the amount of one substance in another. It is the ratio of the amount of the substance of interest to the amount of that substance plus the amount of the substance." [Wikipedia:Wikipedia]
is_a: UO:0000186 ! dimensionless unit

[Term]
id: UO:0000167
name: parts per hundred
def: "A dimensionless concentration notation which denotes the amount of a given substance in a total amount of 100 regardless of the units of measure as long as they are the same." [UOC:GVG]
synonym: "10^[-2]" EXACT []
synonym: "pph" EXACT []
is_a: UO:1000167 ! parts per hundred based unit

[Term]
id: UO:0000168
name: parts per thousand
def: "A dimensionless concentration notation which denotes the amount of a given substance in a total amount of 1000 regardless of the units of measure as long as they are the same." [UOC:GVG]
synonym: "10^[-3]" EXACT []
synonym: "ppth" EXACT []
is_a: UO:1000168 ! parts per thousand based unit

[Term]
id: UO:0000169
name: parts per million
def: "A dimensionless concentration notation which denotes the amount of a given substance in a total amount of 1,000,000 regardless of the units of measure used as long as they are the same or 1 part in 10^[6]." [UOC:GVG]
synonym: "10^[-6]" EXACT []
synonym: "ppm" EXACT []
is_a: UO:1000169 ! parts per million based unit

[Term]
id: UO:0000170
name: parts per billion
def: "A dimensionless concentration notation which denotes the amount of a given substance in a total amount of 1,000,000,000 regardless of the units of measure as long as they are the same or 1 part in 10^[9]." [UOC:GVG]
synonym: "10^[-9]" EXACT []
synonym: "ppb" EXACT []
is_a: UO:1000170 ! parts per billion based unit

[Term]
id: UO:0000171
name: parts per trillion
def: "A dimensionless concentration notation which denotes the amount of a given substance in a total amount of 1,000,000,000 regardless of the units of measure used as long as they are the same or 1 part in 10^[12]." [UOC:GVG]
synonym: "10^[-12]" EXACT []
synonym: "ppt" EXACT []
is_a: UO:1000171 ! parts per trillion based unit

[Term]
id: UO:0000172
name: parts per quadrillion
def: "A dimensionless concentration notation which denotes the amount of a given substance in a total amount of 1,000,000,000,000 regardless of the units of measure used as long as they are the same or 1 part in 10^[15]." [UOC:GVG]
synonym: "10^[-15]" EXACT []
synonym: "ppq" EXACT []
is_a: UO:1000172 ! parts per quadrillion based unit

[Term]
id: UO:0000173
name: gram per milliliter
def: "A mass unit density which is equal to mass of an object in grams divided by the volume in milliliter." [UOC:GVG]
synonym: "g/ml" EXACT []
synonym: "gram per millilitre" EXACT []
is_a: UO:1000173 ! gram per milliliter based unit

[Term]
id: UO:0000174
name: kilogram per liter
def: "A mass unit density which is equal to mass of an object in kilograms divided by the volume in liters." [UOC:GVG]
synonym: "kg/L" EXACT []
synonym: "kilogram per litre" EXACT []
is_a: UO:1000175 ! gram per liter based unit
intersection_of: UO:1000175 ! gram per liter based unit
intersection_of: has:prefix UO:0000294 ! kilo
relationship: has:prefix UO:0000294 ! kilo

[Term]
id: UO:0000175
name: gram per liter
def: "A mass unit density which is equal to mass of an object in grams divided by the volume in liters." [UOC:GVG]
synonym: "g/L" EXACT []
synonym: "gram per litre" EXACT []
is_a: UO:1000175 ! gram per liter based unit

[Term]
id: UO:0000176
name: milligram per milliliter
def: "A mass unit density which is equal to mass of an object in milligrams divided by the volume in milliliters." [UOC:GVG]
synonym: "mg/ml" EXACT []
synonym: "milligram per millilitre" EXACT []
is_a: UO:1000173 ! gram per milliliter based unit
intersection_of: UO:1000173 ! gram per milliliter based unit
intersection_of: has:prefix UO:0000297 ! milli
relationship: has:prefix UO:0000297 ! milli

[Term]
id: UO:0000177
name: unit per volume unit
def: "A concentration unit which is a standard measure of the number of units, as an agreed arbitrary amount, of a given substance per a specific volume of solution." [Webmd:Webmd]
is_a: UO:0000051 ! concentration unit

[Term]
id: UO:0000178
name: unit per milliliter
def: "A unit per milliliter unit which is equal to one unit of an agreed arbitrary amount per one milliliter." [Webmd:Webmd]
synonym: "U/ml" EXACT []
synonym: "unit per millilitre" EXACT []
is_a: UO:1000178 ! unit per milliliter based unit

[Term]
id: UO:0000179
name: unit per liter
def: "A unit per milliliter unit which is equal to one unit of an agreed arbitrary amount per one liter." [UOC:GVG]
synonym: "U/l" EXACT []
synonym: "unit per litre" EXACT []
is_a: UO:1000179 ! unit per liter based unit

[Term]
id: UO:0000180
name: mass per unit volume
def: "A concentration unit which is a standard measure of the mass of a substance in a given volume (density)." [Wikipedia:Wikipedia]
is_a: UO:1000180 ! mass per unit volume based unit

[Term]
id: UO:0000181
name: enzyme unit
def: "A catalytic unit activity which is equal to the amount of the enzyme that catalyzes the conversion of 1 micro mole of substrate per minute." [Wikipedia:Wikipedia]
synonym: "U" EXACT []
is_a: UO:1000181 ! enzyme unit based unit

[Term]
id: UO:0000182
name: density unit
def: "A unit which is a standard measure of the influence exerted by some mass." [Wikipedia:Wikipedia]
is_a: UO:0000000 ! unit

[Term]
id: UO:0000183
name: linear density unit
def: "A density unit which is a standard measure of the mass exerting an influence on a one-dimensional object." [Wikipedia:Wikipedia]
is_a: UO:0000182 ! density unit

[Term]
id: UO:0000184
name: kilogram per meter
def: "An area density unit which is equal to the mass of an object in kilograms divided by one meter." [NIST:NIST]
synonym: "kg/m" EXACT []
synonym: "kilogram per metre" EXACT []
is_a: UO:0000183 ! linear density unit

[Term]
id: UO:0000185
name: degree
def: "A plane angle unit which is equal to 1/360 of a full rotation or 1.7453310^[-2] rad." [Wikipedia:Wikipedia]
is_a: UO:1000185 ! degree based unit

[Term]
id: UO:0000186
name: dimensionless unit
def: "A unit which is a standard measure of physical quantity consisting of only a numerical number without any units." [Wikipedia:Wikipedia]
is_a: UO:0000000 ! unit

[Term]
id: UO:0000187
name: percent
def: "A dimensionless ratio unit which denotes numbers as fractions of 100." [Wikipedia:Wikipedia]
synonym: "%" EXACT []
is_a: UO:0000190 ! ratio unit

[Term]
id: UO:0000188
name: pi
def: "A dimensionless unit which denoted an irrational real number, approximately equal to 3.14159 which is the ratio of a circle's circumference to its diameter in Euclidean geometry." [Wikipedia:Wikipedia]
is_a: UO:1000188 ! pi based unit

[Term]
id: UO:0000189
name: count unit
def: "A dimensionless unit which denotes a simple count of things." [MGED:MGED]
synonym: "count" EXACT []
is_a: UO:0000186 ! dimensionless unit

[Term]
id: UO:0000190
name: ratio unit
def: "A dimensionless unit which denotes an amount or magnitude of one quantity relative to another." [Wikipedia:Wikipedia]
is_a: UO:0000186 ! dimensionless unit

[Term]
id: UO:0000191
name: fraction
def: "A dimensionless ratio unit which relates the part (the numerator) to the whole (the denominator)." [Wikipedia:Wikipedia]
is_a: UO:0000190 ! ratio unit

[Term]
id: UO:0000192
name: molecule count
def: "A dimensionless count unit which denotes the number of molecules." [MGED:MGED]
is_a: UO:1000192 ! molecule count based unit

[Term]
id: UO:0000193
name: purity percentage
def: "A dimensionless percent unit which denotes the homogeneity of a biomaterial." [MGED:MGED]
is_a: UO:1000193 ! purity percentage based unit

[Term]
id: UO:0000194
name: confluence percentage
def: "A dimensionless percent unit which denotes the density of an attached or monolayer culture (e.g., cell culture)." [MGED:MGED]
is_a: UO:1000194 ! confluence percentage based unit

[Term]
id: UO:0000195
name: degree Fahrenheit
def: "A temperature unit which is equal to 5/9ths of a kelvin. Negative 40 degrees Fahrenheit is equal to negative 40 degrees Celsius." [Wikipedia:Wikipedia]
synonym: "F" EXACT []
is_a: UO:1000195 ! degree Fahrenheit based unit

[Term]
id: UO:0000196
name: pH
def: "A dimensionless concentration notation which denotes the acidity of a solution in terms of activity of hydrogen ions (H+)." [Wikipedia:Wikipedia]
is_a: UO:1000196 ! pH based unit

[Term]
id: UO:0000197
name: liter per kilogram
def: "A specific volume unit which is equal to one liter volume occupied by one kilogram of a particular substance." [NIST:NIST]
synonym: "l/kg" EXACT []
synonym: "litre per kilogram" EXACT []
is_a: UO:1000197 ! liter per kilogram based unit

[Term]
id: UO:0000198
name: milliliter per kilogram
def: "A specific volume unit which is equal to a thousandth of a liter per kilogram or 10^[-3] l/kg." [NIST:NIST]
synonym: "millilitre per kilogram" EXACT []
synonym: "ml/kg" EXACT []
is_a: UO:1000197 ! liter per kilogram based unit
intersection_of: UO:1000197 ! liter per kilogram based unit
intersection_of: has:prefix UO:0000297 ! milli
relationship: has:prefix UO:0000297 ! milli

[Term]
id: UO:0000199
name: microliter per kilogram
def: "A specific volume unit which is equal to one millionth of a liter per kilogram or 10^[-6] l/kg." [NIST:NIST]
synonym: "microlitre per kilogram" EXACT []
synonym: "ul/kg" EXACT []
is_a: UO:1000197 ! liter per kilogram based unit
intersection_of: UO:1000197 ! liter per kilogram based unit
intersection_of: has:prefix UO:0000299 ! micro
relationship: has:prefix UO:0000299 ! micro

[Term]
id: UO:0000200
name: cell concentration unit
def: "A concentration unit which denotes the average cell number in a given volume." [Bioedonline:Bioedonline]
is_a: UO:0000051 ! concentration unit

[Term]
id: UO:0000201
name: cells per milliliter
def: "A unit of cell concentration which is equal to one cell in a volume of 1 milliliter." [Bioedonline:Bioedonline]
synonym: "cells per millilitre" EXACT []
synonym: "cells per ml" EXACT []
is_a: UO:1000201 ! cells per milliliter based unit

[Term]
id: UO:0000202
name: catalytic (activity) concentration unit
def: "A concentration unit which is a standard measure of the amount of the action of a catalyst in a given volume." [UOC:GVG]
is_a: UO:0000051 ! concentration unit

[Term]
id: UO:0000203
name: katal per cubic meter
def: "A catalytic (activity) concentration unit which is equal to 1 katal activity of a catalyst in a given volume of one cubic meter." [NIST:NIST]
synonym: "kat/m^[3]" EXACT []
synonym: "katal per cubic metre" EXACT []
is_a: UO:1000203 ! katal per cubic meter based unit

[Term]
id: UO:0000204
name: katal per liter
def: "A catalytic (activity) concentration unit which is equal to 1 katal activity of a catalyst in a given volume of one thousandth of a cubic meter." [NIST:NIST]
synonym: "kat/l" EXACT []
synonym: "katal per litre" EXACT []
is_a: UO:1000204 ! katal per liter based unit

[Term]
id: UO:0000205
name: volume per unit volume
def: "A dimensionless concentration unit which denotes the given volume of the solute in the total volume of the resulting solution." [NIST:NIST]
is_a: UO:0000051 ! concentration unit

[Term]
id: UO:0000206
name: milliliter per cubic meter
def: "A volume per unit volume unit which is equal to one millionth of a liter of solute in one cubic meter of solution." [NIST:NIST]
synonym: "millilitre per cubic metre" EXACT []
synonym: "ml/m^[3]" EXACT []
is_a: UO:0000205 ! volume per unit volume

[Term]
id: UO:0000207
name: milliliter per liter
def: "A volume per unit volume unit which is equal to one millionth of a liter of solute in one liter of solution." [NIST:NIST]
synonym: "millilitre per litre" EXACT []
synonym: "ml/l" EXACT []
is_a: UO:0000205 ! volume per unit volume

[Term]
id: UO:0000208
name: gram per deciliter
def: "A mass density unit which is equal to mass of an object in grams divided by the volume in deciliters." [UOC:GVG]
synonym: "g/dl" EXACT []
synonym: "gram per decilitre" EXACT []
is_a: UO:1000208 ! gram per deciliter based unit

[Term]
id: UO:0000209
name: deciliter
def: "A volume unit which is equal to one tenth of a liter or 10^[-1] L." [NIST:NIST]
synonym: "decilitre" EXACT []
synonym: "dl" EXACT []
is_a: UO:1000099 ! liter based unit
intersection_of: UO:1000099 ! liter based unit
intersection_of: has:prefix UO:0000296 ! deci
relationship: has:prefix UO:0000296 ! deci

[Term]
id: UO:0000210
name: colony forming unit
def: "A dimensionless count unit which a measure of viable bacterial numbers." [Wikipedia:Wikipedia]
synonym: "cfu" EXACT []
is_a: UO:1000210 ! colony forming unit based unit

[Term]
id: UO:0000211
name: plaque forming unit
def: "A dimensionless count unit which a measure of plaque forming units in a given volume." [Wikipedia:Wikipedia]
synonym: "pfu" EXACT []
is_a: UO:1000211 ! plaque forming unit based unit

[Term]
id: UO:0000212
name: colony forming unit per volume
def: "A concentration unit which a measure of viable bacterial numbers in a given volume." [Wikipedia:Wikipedia]
is_a: UO:0000051 ! concentration unit

[Term]
id: UO:0000213
name: colony forming unit per milliliter
def: "A colony forming unit which a measure of viable bacterial numbers in one milliliter." [Wikipedia:Wikipedia]
synonym: "cfu/ml" EXACT []
synonym: "colony forming unit per millilitre" EXACT []
is_a: UO:1000213 ! colony forming unit per milliliter based unit

[Term]
id: UO:0000214
name: plaque forming unit per volume
def: "A concentration unit which a measure of plaque forming units in a given volume." [UOC:GVG]
is_a: UO:0000051 ! concentration unit

[Term]
id: UO:0000215
name: plaque forming unit per milliliter
def: "A concentration unit which a measure of plaque forming units in one milliliter." [UOC:GVG]
synonym: "pfu/ml" EXACT []
synonym: "plaque forming unit per millilitre" EXACT []
is_a: UO:1000215 ! plaque forming unit per milliliter based unit

[Term]
id: UO:0000216
name: disintegrations per second
def: "An activity (of a radionuclide) unit which is equal to the activity of a quantity of radioactive material in which one nucleus decays per second or there is one atom disintegration per second." [ORCBS:ORCBS]
synonym: "dps" EXACT []
is_a: UO:1000216 ! disintegrations per second based unit

[Term]
id: UO:0000217
name: electric potential difference unit
def: "A unit which is a standard measure of the work done per unit charge as a charge is moved between two points in an electric field." [Wikipedia:Wikipedia]
is_a: UO:0000000 ! unit

[Term]
id: UO:0000218
name: volt
def: "An electric potential difference unit which is equal to the work per unit charge. One volt is the potential difference required to move one coulomb of charge between two points in a circuit while using one joule of energy." [Wikipedia:Wikipedia]
synonym: "V" EXACT []
is_a: UO:1000218 ! volt based unit

[Term]
id: UO:0000219
name: electric charge
def: "A unit which is a standard measure of the quantity of unbalanced electricity in a body (either positive or negative) and construed as an excess or deficiency of electrons." [WordNet:WordNet]
is_a: UO:0000000 ! unit

[Term]
id: UO:0000220
name: coulomb
def: "An electrical charge unit which is equal to the amount of charge transferred by a current of 1 ampere in 1 second." [WordNet:WordNet]
synonym: "C" EXACT []
is_a: UO:1000220 ! coulomb based unit

[Term]
id: UO:0000221
name: dalton
def: "An independently to the base SI units defined mass unit which is equal to one twelfth of the mass of an unbound atom of the carbon-12 nuclide, at rest and in its ground state." [Wikipedia:Wikipedia]
synonym: "amu" EXACT []
synonym: "Da" EXACT []
synonym: "u" EXACT []
synonym: "unified atomic mass unit" EXACT []
is_a: UO:1000221 ! dalton based unit

[Term]
id: UO:0000222
name: kilodalton
def: "A mass unit which is equal to one thousand daltons." [Wikipedia:Wikipedia]
synonym: "kDa" EXACT []
is_a: UO:1000221 ! dalton based unit
intersection_of: UO:1000221 ! dalton based unit
intersection_of: has:prefix UO:0000294 ! kilo
relationship: has:prefix UO:0000294 ! kilo

[Term]
id: UO:0000223
name: watt-hour
def: "An energy unit which is equal to the amount of electrical energy equivalent to a one-watt load drawing power for one hour." [Wikipedia:Wikipedia]
synonym: "Wh" EXACT []
is_a: UO:1000223 ! watt-hour based unit

[Term]
id: UO:0000224
name: kilowatt-hour
def: "An energy unit which is equal to 1,000 watt-hours." [Wikipedia:Wikipedia]
is_a: UO:1000223 ! watt-hour based unit
intersection_of: UO:1000223 ! watt-hour based unit
intersection_of: has:prefix UO:0000294 ! kilo
relationship: has:prefix UO:0000294 ! kilo

[Term]
id: UO:0000225
name: magnetic flux unit
def: "A unit which is a standard measure of quantity of magnetism, taking account of the strength and the extent of a magnetic field." [Wikipedia:Wikipedia]
is_a: UO:0000000 ! unit

[Term]
id: UO:0000226
name: weber
def: "A magnetic flux unit which is equal to the amount of flux that when linked with a single turn of wire for an interval of one second will induce an electromotive force of one volt." [ScienceLobby:ScienceLobby]
synonym: "V s" EXACT []
synonym: "volt-second" RELATED []
synonym: "Wb" EXACT []
is_a: UO:1000226 ! weber based unit

[Term]
id: UO:0000227
name: magnetic flux density unit
def: "A unit which is a standard measure of the strength of a magnetic field." [allnet:allnet]
synonym: "B" EXACT []
is_a: UO:0000000 ! unit

[Term]
id: UO:0000228
name: tesla
def: "A magnetic flux density unit which is equal to one weber per square meter." [WordNet:WordNet]
synonym: "T" EXACT []
synonym: "Wb/m2" EXACT []
is_a: UO:1000228 ! tesla based unit

[Term]
id: UO:0000229
name: volt-hour
def: "A magnetic flux unit which is equal to 3600 Wb." [UOC:GVG]
synonym: "Vh" EXACT []
is_a: UO:1000229 ! volt-hour based unit

[Term]
id: UO:0000230
name: kilovolt-hour
def: "A magnetic flux unit which is equal to one thousand volt-hours." [UOC:GVG]
synonym: "kVh" EXACT []
is_a: UO:1000229 ! volt-hour based unit
intersection_of: UO:1000229 ! volt-hour based unit
intersection_of: has:prefix UO:0000294 ! kilo
relationship: has:prefix UO:0000294 ! kilo

[Term]
id: UO:0000231
name: information unit
def: "A unit which is a standard measure of the amount of information." [Wikipedia:Wikipedia]
is_a: UO:0000000 ! unit

[Term]
id: UO:0000232
name: bit
def: "An information unit which refers to a digit in the binary numeral system, which consists of base 2 digits (ie there are only 2 possible values: 0 or 1)." [Wikipedia:Wikipedia]
is_a: UO:1000232 ! bit based unit

[Term]
id: UO:0000233
name: byte
def: "An information unit which is equal to 8 bits." [Wikipedia:Wikipedia]
synonym: "B" EXACT []
is_a: UO:1000233 ! byte based unit

[Term]
id: UO:0000234
name: kilobyte
def: "An information unit which is equal to 1000 bytes." [Wikipedia:Wikipedia]
synonym: "kB" EXACT []
is_a: UO:1000233 ! byte based unit
intersection_of: UO:1000233 ! byte based unit
intersection_of: has:prefix UO:0000294 ! kilo
relationship: has:prefix UO:0000294 ! kilo

[Term]
id: UO:0000235
name: megabyte
def: "An information unit which is equal to 1000 kB." [Wikipedia:Wikipedia]
synonym: "MB" EXACT []
is_a: UO:1000233 ! byte based unit
intersection_of: UO:1000233 ! byte based unit
intersection_of: has:prefix UO:0000293 ! mega
relationship: has:prefix UO:0000293 ! mega

[Term]
id: UO:0000236
name: image resolution unit
def: "An information unit which is a standard measure of the detail an image holds." [Wikipedia:Wikipedia]
is_a: UO:0000231 ! information unit

[Term]
id: UO:0000237
name: chroma sampling unit
def: "An image resolution unit which is a standard measure of the amount of spatial detail in an image." [Wikipedia:Wikipedia]
is_a: UO:1000237 ! chroma sampling unit based unit

[Term]
id: UO:0000238
name: dynamic range unit
def: "An image resolution unit which is a standard measure of the amount of contrast available in a pixel." [Wikipedia:Wikipedia]
is_a: UO:1000238 ! dynamic range unit based unit

[Term]
id: UO:0000239
name: spatial resolution unit
def: "An image resolution unit which is a standard measure of the way luminance and chrominance may be sampled at different levels." [Wikipedia:Wikipedia]
is_a: UO:0000236 ! image resolution unit

[Term]
id: UO:0000240
name: dots per inch
def: "A spatial resolution unit which is a standard measure of the printing resolution, in particular the number of individual dots of ink a printer or toner can produce within a linear one-inch space." [Wikipedia:Wikipedia]
synonym: "dpi" EXACT []
is_a: UO:1000240 ! dots per inch based unit

[Term]
id: UO:0000241
name: micron pixel
def: "A spatial resolution unit which is equal to a pixel size of one micrometer." [Wikipedia:Wikipedia]
synonym: "micrometer pixel" EXACT []
is_a: UO:0000239 ! spatial resolution unit

[Term]
id: UO:0000242
name: pixels per inch
def: "A spatial resolution unit which is a standard measure of the resolution of a computer display, related to the size of the display in inches and the total number of pixels in the horizontal and vertical directions." [Wikipedia:Wikipedia]
synonym: "pixel density" EXACT []
synonym: "ppi" EXACT []
is_a: UO:1000242 ! pixels per inch based unit

[Term]
id: UO:0000243
name: pixels per millimeter
def: "A spatial resolution unit which is a standard measure of the number of pixels in one millimeter length or width of a digital image divided by the physical length or width of a printed image." [Wikipedia:Wikipedia]
synonym: "pixels per millimetre" EXACT []
is_a: UO:1000243 ! pixels per millimeter based unit

[Term]
id: UO:0000244
name: base pair
def: "A count unit which contains one nucleotide." [UO:GVG]
synonym: "basepair" EXACT []
synonym: "bp" EXACT []
is_a: UO:1000244 ! base pair based unit

[Term]
id: UO:0000245
name: kibibyte
def: "An information unit which is equal to 1024 B." [NIST:NIST]
synonym: "KiB" EXACT []
is_a: UO:1000245 ! kibibyte based unit

[Term]
id: UO:0000246
name: mebibyte
def: "An information unit which is equal to 1024 KiB." [NIST:NIST]
synonym: "MiB" EXACT []
is_a: UO:1000246 ! mebibyte based unit

[Term]
id: UO:0000247
name: millivolt
def: "An electric potential difference unit which is equal to one thousandth of a volt or 10^[-3] V." [UOC:GVG]
synonym: "mV" EXACT []
is_a: UO:1000218 ! volt based unit
intersection_of: UO:1000218 ! volt based unit
intersection_of: has:prefix UO:0000297 ! milli
relationship: has:prefix UO:0000297 ! milli

[Term]
id: UO:0000248
name: kilovolt
def: "An electric potential difference unit which is equal to one thousand volts or 10^[3] V." [UOC:GVG]
synonym: "kV" EXACT []
is_a: UO:1000218 ! volt based unit
intersection_of: UO:1000218 ! volt based unit
intersection_of: has:prefix UO:0000294 ! kilo
relationship: has:prefix UO:0000294 ! kilo

[Term]
id: UO:0000249
name: microvolt
def: "An electric potential difference unit which is equal to one millionth of a volt or 10^[-6] V." [UOC:GVG]
synonym: "uV" EXACT []
is_a: UO:1000218 ! volt based unit
intersection_of: UO:1000218 ! volt based unit
intersection_of: has:prefix UO:0000299 ! micro
relationship: has:prefix UO:0000299 ! micro

[Term]
id: UO:0000250
name: nanovolt
def: "An electric potential difference unit which is equal to one billionth of a volt or 10^[-12] V." [UOC:GVG]
synonym: "nV" EXACT []
is_a: UO:1000218 ! volt based unit
intersection_of: UO:1000218 ! volt based unit
intersection_of: has:prefix UO:0000300 ! nano
relationship: has:prefix UO:0000300 ! nano

[Term]
id: UO:0000251
name: picovolt
def: "An electric potential difference unit which is equal to one trillionth of a volt or 10^[-12] V." [UOC:GVG]
synonym: "pV" EXACT []
is_a: UO:1000218 ! volt based unit
intersection_of: UO:1000218 ! volt based unit
intersection_of: has:prefix UO:0000302 ! pico
relationship: has:prefix UO:0000302 ! pico

[Term]
id: UO:0000252
name: megavolt
def: "An electric potential difference unit which is equal to one million volts or 10^[6] V." [UOC:GVG]
synonym: "MV" EXACT []
is_a: UO:1000218 ! volt based unit
intersection_of: UO:1000218 ! volt based unit
intersection_of: has:prefix UO:0000293 ! mega
relationship: has:prefix UO:0000293 ! mega

[Term]
id: UO:0000253
name: surface tension unit
def: "A unit which is a standard measure of the ability of a liguid to attraction of molecules at its surface as a result of unbalanced molecular cohesive forces." [NIST:NIST]
is_a: UO:0000000 ! unit

[Term]
id: UO:0000254
name: newton per meter
def: "A surface tension unit which is equal to one newton per meter." [NIST:NIST]
synonym: "N/m" EXACT []
synonym: "newton per metre" EXACT []
is_a: UO:1000254 ! newton per meter based unit

[Term]
id: UO:0000255
name: dyne per cm
def: "A surface tension unit which is equal to one dyne per centimeter." [Wikipedia:Wikipedia]
synonym: "dyn/cm" EXACT []
is_a: UO:1000255 ! dyne per cm based unit

[Term]
id: UO:0000256
name: viscosity unit
def: "A unit which is a standard measure of the internal resistance of fluids to flow." [UOC:GVG]
is_a: UO:0000000 ! unit

[Term]
id: UO:0000257
name: pascal second
def: "A viscosity unit which is equal to one pascale per second." [NIST:NIST]
synonym: "Pa  s" EXACT []
is_a: UO:1000257 ! pascal second based unit

[Term]
id: UO:0000258
name: poise
def: "A viscosity unit which is equal to one dyne second per square centimeter." [Wikipedia:Wikipedia]
synonym: "dyne s/cm^2" EXACT []
synonym: "P" EXACT []
is_a: UO:1000258 ! poise based unit

[Term]
id: UO:0000259
name: decibel
def: "A ratio unit which is an indicator of sound power per unit area." [techtarget:techtarget]
synonym: "dB" EXACT []
is_a: UO:0000190 ! ratio unit

[Term]
id: UO:0000260
name: effective dose unit
def: "A unit which is a standard measure of the estimate of the stochastic effect that a non-uniform radiation dose has on a human." [Wikipedia:Wikipedia]
is_a: UO:1000260 ! effective dose unit based unit

[Term]
id: UO:0000261
name: conduction unit
def: "A unit which represents a standard measurement of the transmission of an entity through a medium." [UOC:GVG]
is_a: UO:0000000 ! unit

[Term]
id: UO:0000262
name: electrical conduction unit
def: "A unit which represents a standard measurement of the movement of electrically charged particles through a transmission medium (electrical conductor)." [UOC:GVG]
is_a: UO:0000261 ! conduction unit

[Term]
id: UO:0000263
name: heat conduction unit
def: "A unit which represents a standard measurement of the spontaneous transfer of thermal energy through matter, from a region of higher temperature to a region of lower temperature." [Wikipedia:Wikipedia]
is_a: UO:0000261 ! conduction unit

[Term]
id: UO:0000264
name: siemens
def: "An electrical conduction unit which is equal to A/V." [NIST:NIST]
synonym: "A V^-1" EXACT []
synonym: "mho " EXACT []
synonym: "S" RELATED []
is_a: UO:1000264 ! siemens based unit

[Term]
id: UO:0000265
name: watt per meter kelvin
def: "An heat conduction unit which is equal to one watt divided by meter kelvin." [NIST:NIST]
synonym: "W/m K" EXACT []
synonym: "watt per metre kelvin" EXACT []
is_a: UO:1000265 ! watt per meter kelvin based unit

[Term]
id: UO:0000266
name: electronvolt
def: "A non-SI unit of energy (eV) defined as the energy acquired by a single unbound electron when it passes through an electrostatic potential difference of one volt. An electronvolt is equal to 1.602 176 53(14) x 10^-19 J." [Wikipedia:Wikipedia]
synonym: "electron volt" EXACT []
synonym: "eV" EXACT []
is_a: UO:1000266 ! electronvolt based unit

[Term]
id: UO:0000267
name: electric field strength unit
def: "The electric field strength is a unit which is a measure of the potential difference between two points some distance apart." [Wikipedia:Electric_field]
synonym: "E-field strength " EXACT []
is_a: UO:0000000 ! unit

[Term]
id: UO:0000268
name: volt per meter
def: "The volt per meter is a unit of electric field strength equal to the a potential difference of 1 volt existing between two points that are 1 meter apart." [Wikipedia:Electric_field]
synonym: "V/m" EXACT []
synonym: "volt per metre" EXACT []
is_a: UO:1000268 ! volt per meter based unit

[Term]
id: UO:0000269
name: absorbance unit
def: "A dimensionless logarithmic unit assigned to a measure of absorbance of light through a partially absorbing substance, defined as -log10(I/I_0) where I = transmitted light and I_0 = incident light." [Wikipedia:Absorbance]
synonym: "AU" EXACT []
is_a: UO:1000269 ! absorbance unit based unit

[Term]
id: UO:0000270
name: volumetric flow rate unit
def: "A unit which is a standard measure of the volume of fluid which passes through a given surface per unit time ." [Wikipedia:Wikipedia]
is_a: UO:0000000 ! unit

[Term]
id: UO:0000271
name: microliters per minute
def: "A volumetric flow rate unit which is equal to one microliter volume through a given surface in one minute." [UOC:GVG]
synonym: "microlitres per minute" EXACT []
synonym: "uL/min" EXACT []
is_a: UO:0000270 ! volumetric flow rate unit

[Term]
id: UO:0000272
name: millimetres of mercury
def: "A unit of pressure equal to the amount of fluid pressure one millimeter deep in mercury at zero degrees centigrade on Earth." [url:en.wiktionary.org/wiki/mmHg]
synonym: "millimeters of mercury" EXACT []
synonym: "mmHg" EXACT []
is_a: UO:0000109 ! pressure unit

[Term]
id: UO:0000273
name: milligram per liter
def: "A mass unit density which is equal to mass of an object in milligrams divided by the volume in liters." [UOC:GVG]
synonym: "mg/L" EXACT []
synonym: "milligram per litre" EXACT []
is_a: UO:1000175 ! gram per liter based unit
intersection_of: UO:1000175 ! gram per liter based unit
intersection_of: has:prefix UO:0000297 ! milli
relationship: has:prefix UO:0000297 ! milli

[Term]
id: UO:0000274
name: microgram per milliliter
def: "A mass unit density which is equal to mass of an object in micrograms divided by the volume in millliters." [UOC:GVG]
synonym: "microgram per millilitre" EXACT []
synonym: "ug/ml" EXACT []
is_a: UO:1000173 ! gram per milliliter based unit
intersection_of: UO:1000173 ! gram per milliliter based unit
intersection_of: has:prefix UO:0000299 ! micro
relationship: has:prefix UO:0000299 ! micro

[Term]
id: UO:0000275
name: nanogram per milliliter
def: "A mass unit density which is equal to mass of an object in nanograms divided by the volume in milliliters." [UOC:GVG]
synonym: "nanogram per millilitre" EXACT []
synonym: "ng/ml" EXACT []
is_a: UO:1000173 ! gram per milliliter based unit
intersection_of: UO:1000173 ! gram per milliliter based unit
intersection_of: has:prefix UO:0000300 ! nano
relationship: has:prefix UO:0000300 ! nano

[Term]
id: UO:0000276
name: amount per container
def: "A concentration unit which is a standard measure of the amount of a substance in a given container." [UOC:GVG]
is_a: UO:0000051 ! concentration unit

[Term]
id: UO:0000277
name: ug/disk
def: "A unit which is equal to one microgram per disk, where a disk is some physical surface/container upon which the substance is deposited." [UOC:MD]
is_a: UO:0000276 ! amount per container

[Term]
id: UO:0000278
name: nmole/disk
def: "A unit which is equal to one nanomole per disk, where a disk is some physical surface/container upon which the substance is deposited." [UOC:MD]
is_a: UO:0000276 ! amount per container

[Term]
id: UO:0000279
name: milliunits per milliliter
def: "A unit per milliliter unit which is equal to one thousandth of a unit of an agreed arbitrary amount per one milliliter." [UOC:GVG]
synonym: "milliunits per millilitre" EXACT []
synonym: "mU/ml" EXACT []
is_a: UO:0000177 ! unit per volume unit

[Term]
id: UO:0000280
name: rate unit
def: "A unit which represents a standard measurement occurrence of a process per unit time." [UOC:GVG]
is_a: UO:0000000 ! unit

[Term]
id: UO:0000281
name: count per nanomolar second
def: "A rate unit which is equal to one over one nanomolar second." [UOC:GVG]
synonym: "nM^-1 s^-1" EXACT []
is_a: UO:1000281 ! count per nanomolar second based unit

[Term]
id: UO:0000282
name: count per molar second
def: "A rate unit which is equal to one over one molar second." [UOC:GVG]
synonym: "M^-1 s^-1" EXACT []
is_a: UO:1000282 ! count per molar second based unit

[Term]
id: UO:0000283
name: kilogram per hectare
def: "An area density unit which is equal to the mass of an object in kilograms divided by the surface area in hectares." [UO:GVG]
is_a: UO:0000054 ! area density unit

[Term]
id: UO:0000284
name: count per nanomolar
def: "A rate unit which is equal to one over one nanomolar." [UO:GVG]
synonym: "1/nM" EXACT []
synonym: "nM^-1" EXACT []
is_a: UO:1000284 ! count per nanomolar based unit

[Term]
id: UO:0000285
name: count per molar
def: "A rate unit which is equal to one over one molar." [UO:GVG]
synonym: "1/M" EXACT []
synonym: "M^-1" EXACT []
is_a: UO:1000285 ! count per molar based unit

[Term]
id: UO:0000286
name: yotta
def: "A prefix in the metric system denoting a factor of ten to the power of 24." [UO:GVG]
synonym: "10^[24]" EXACT []
synonym: "Y" EXACT []
is_a: UO:0000046 ! prefix

[Term]
id: UO:0000287
name: hecto
def: "A prefix in the metric system denoting a factor of one hundred." [UO:GVG]
synonym: "10^[2]" EXACT []
synonym: "h" EXACT []
is_a: UO:0000046 ! prefix

[Term]
id: UO:0000288
name: zetta
def: "A prefix in the metric system denoting a factor of ten to the power of 21." [UO:GVG]
synonym: "10^[21]" EXACT []
synonym: "Z" EXACT []
is_a: UO:0000046 ! prefix

[Term]
id: UO:0000289
name: exa
def: "A prefix in the metric system denoting a factor of ten to the power of 18." [UO:GVG]
synonym: "10^[18]" EXACT []
synonym: "E" EXACT []
is_a: UO:0000046 ! prefix

[Term]
id: UO:0000290
name: peta
def: "A prefix in the metric system denoting a factor of ten to the power of 15." [UO:GVG]
synonym: "10^[15]" EXACT []
synonym: "P" EXACT []
is_a: UO:0000046 ! prefix

[Term]
id: UO:0000291
name: tera
def: "A prefix in the metric system denoting a factor of ten to the power of 12." [UO:GVG]
synonym: "10^[12]" RELATED []
synonym: "T" EXACT []
is_a: UO:0000046 ! prefix

[Term]
id: UO:0000292
name: giga
def: "A prefix in the metric system denoting a factor of ten to the power of 9." [UO:GVG]
synonym: "10^[9]" EXACT []
synonym: "G" EXACT []
is_a: UO:0000046 ! prefix

[Term]
id: UO:0000293
name: mega
def: "A prefix in the metric system denoting a factor of million." [UO:GVG]
synonym: "10^[6]" EXACT []
synonym: "M" EXACT []
is_a: UO:0000046 ! prefix

[Term]
id: UO:0000294
name: kilo
def: "A prefix in the metric system denoting a factor of one thousand." [UO:GVG]
synonym: "10^[3]" EXACT []
synonym: "k" EXACT []
is_a: UO:0000046 ! prefix

[Term]
id: UO:0000295
name: deca
def: "A prefix in the metric system denoting a factor of ten." [UO:GVG]
synonym: "10^[1]" EXACT []
synonym: "da" EXACT []
is_a: UO:0000046 ! prefix

[Term]
id: UO:0000296
name: deci
def: "A prefix in the metric system denoting a factor of one tenth." [UO:GVG]
synonym: "10^[-1]" EXACT []
synonym: "d" EXACT []
is_a: UO:0000046 ! prefix

[Term]
id: UO:0000297
name: milli
def: "A prefix in the metric system denoting a factor of one thousand." [UO:GVG]
synonym: "10^[-3]" EXACT []
synonym: "m" EXACT []
is_a: UO:0000046 ! prefix

[Term]
id: UO:0000298
name: centi
def: "A prefix in the metric system denoting a factor of one hundred." [UO:GVG]
synonym: "10^[-2]" EXACT []
synonym: "c" EXACT []
is_a: UO:0000046 ! prefix

[Term]
id: UO:0000299
name: micro
def: "A prefix in the metric system denoting a factor of 10 to the power of -6." [UO:GVG]
synonym: "10^[-6]" EXACT []
is_a: UO:0000046 ! prefix

[Term]
id: UO:0000300
name: nano
def: "A prefix in the metric system denoting a factor of 10 to the power of -9." [UO:GVG]
synonym: "10^[-9]" EXACT []
synonym: "n" EXACT []
is_a: UO:0000046 ! prefix

[Term]
id: UO:0000301
name: microgram per liter
def: "A mass unit density which is equal to mass of an object in micrograms divided by the volume in liters." [UOC:GVG]
synonym: "microgram per litre" EXACT []
synonym: "ug/L" EXACT []
is_a: UO:1000175 ! gram per liter based unit
intersection_of: UO:1000175 ! gram per liter based unit
intersection_of: has:prefix UO:0000299 ! micro
relationship: has:prefix UO:0000299 ! micro

[Term]
id: UO:0000302
name: pico
def: "A prefix in the metric system denoting a factor of 10 to the power of -12." [GVG:UO]
synonym: "10^[-12]" EXACT []
synonym: "n" EXACT []
is_a: UO:0000046 ! prefix

[Term]
id: UO:0000303
name: femto
def: "A prefix in the metric system denoting a factor of 10 to the power of -15." [UO:GVG]
synonym: "10^[-15]" EXACT []
synonym: "f" EXACT []
is_a: UO:0000046 ! prefix

[Term]
id: UO:0000304
name: atto
def: "A prefix in the metric system denoting a factor of 10 to the power of -18." [UO:GVG]
synonym: "10^[-18]" RELATED []
synonym: "a" EXACT []
is_a: UO:0000046 ! prefix

[Term]
id: UO:0000305
name: zepto
def: "A prefix in the metric system denoting a factor of 10 to the power of -21." [UO:GVG]
synonym: "10^[-21]" RELATED []
synonym: "z" EXACT []
is_a: UO:0000046 ! prefix

[Term]
id: UO:0000306
name: yocto
def: "A prefix in the metric system denoting a factor of 10 to the power of -24." [UO:GVG]
synonym: "10^[-24]" RELATED []
synonym: "y" EXACT []
is_a: UO:0000046 ! prefix

[Term]
id: UO:0000307
name: dose unit
def: "A concentration unit which is a standard measure of the amount of a toxic or pharmaceutical substance administered to a recipient subject, expressed in terms of the size of the subject." [UO:PC]
is_a: UO:0000051 ! concentration unit

[Term]
id: UO:0000308
name: milligram per kilogram
def: "A dose unit which is equal to 1 milligram of a toxic or pharmaceutical substance per kilogram body weight of the recipient subject." [UO:PC]
is_a: UO:0000307 ! dose unit

[Term]
id: UO:0000309
name: milligram per square meter
def: "A dose unit which is equal to 1 milligram of a toxic or pharmaceutical substance per square meter of surface area of the recipient subject." [UO:PC]
is_a: UO:0000307 ! dose unit
is_a: UO:1010049 ! gram per square meter based unit
intersection_of: UO:1010049 ! gram per square meter based unit
intersection_of: has:prefix UO:0000297 ! milli
relationship: has:prefix UO:0000297 ! milli

[Term]
id: UO:0000310
name: dosage unit
def: "A concentration unit which is a standard measure of the amount of a toxic or pharmaceutical substance administered over time to a recipient subject, expressed in terms of the size of the subject." [UO:PC]
is_a: UO:1000310 ! dosage unit based unit

[Term]
id: UO:0000311
name: milligram per kilogram per day
def: "A dosage unit which is equal to 1 milligram per day of a toxic or pharmaceutical substance per kilogram body weight of the recipient subject." [UO:PC]
is_a: UO:0000310 ! dosage unit

[Term]
id: UO:0000312
name: relative light unit
def: "A derived unit which is a measure of relative light intensity, as typically measured by a luminometer, spectrophotometer, or fluorimeter in biological research applications." [UO:PC]
is_a: UO:1000312 ! relative light unit based unit

[Term]
id: UO:0000313
name: relative luminescence unit
def: "A relative light unit which is a measure of relative luminescence intensity." [UO:PC]
is_a: UO:1000313 ! relative luminescence unit based unit

[Term]
id: UO:0000314
name: relative fluorescence unit
def: "A relative light unit which is a measure of relative fluorescence intensity." [UO:PC]
is_a: UO:1000314 ! relative fluorescence unit based unit

[Term]
id: UO:0000315
name: turbidity unit
def: "A unit used to indicate the clarity of water or other solutions or suspensions, as measured by the ability of the solution or suspension to scatter light of a defined wavelength range." [UO:PC]
is_a: UO:0000000 ! unit

[Term]
id: UO:0000316
name: cells per microliter
def: "A unit of cell concentration which is equal to one cell in a volume of 1 microliter." [UO:GVG]
synonym: "cells per microlitre" EXACT []
synonym: "cells per ul" EXACT []
is_a: UO:0000200 ! cell concentration unit

[Term]
id: UO:0000317
name: cells per well
def: "A unit of cell concentration which is equal to 1 cell in a well or discrete container of arbitrary volume." [UO:PC]
is_a: UO:0000200 ! cell concentration unit

[Term]
id: UO:0000318
name: formazin nephelometric unit
def: "1000 formazin turbidity units (FNU) on the empirical formazin turbidity scale represents reflectance of insol. reaction products of 0.0725 g hydrazine sulfate with 0.7250 g hexamethylenetetramine diluted to 1 L." [AOAC:192]
synonym: "FNU" EXACT []
is_a: UO:0000315 ! turbidity unit

[Term]
id: UO:0000319
name: radioactivity concentration
def: "A concentration unit which is a standard measure of the amount of radioactivity in a given volume." [UO:GVG]
is_a: UO:0000051 ! concentration unit

[Term]
id: UO:0000320
name: curie per liter
def: "A unit of radioactivity concentration which is equal to one curie in a volume of 1 liter." [UO:GVG]
synonym: "curie per litre" EXACT []
is_a: UO:0000319 ! radioactivity concentration

[Term]
id: UO:0000321
name: microcurie per milliliter
def: "A unit of radioactivity concentration which is equal to one micro curie in a volume of 1 liter." [UO:GVG]
synonym: "microcurie per millilitre" EXACT []
is_a: UO:0000319 ! radioactivity concentration

[Term]
id: UO:0000322
name: fold dilution
def: "A unit that is the ratio of concentration of two solutions of interest, typically with one solution derived from the other by the addition of solvent." [UO:PC]
is_a: UO:0000186 ! dimensionless unit

[Term]
id: UO:0000323
name: ton per hectare
def: "An area density unit which is equal to the mass of an object in tons divided by the surface area in hectares." [UO:GVG]
is_a: UO:0000054 ! area density unit

[Term]
id: UO:0000324
name: square angstrom
def: "An area unit which is equal to an area enclosed by a square with sides each 1 angstrom long." [UOC:GVG]
synonym: "A^[2]" RELATED []
is_a: UO:0000047 ! area unit

[Term]
id: UO:0000325
name: megaHertz
def: "A frequency unit which is equal to one million hertz or 10^[6] V." [UOC:GVG]
synonym: "megahertz" RELATED []
synonym: "mH" RELATED []
is_a: UO:0000105 ! frequency unit

[Term]
id: UO:0000326
name: centiMorgan
def: "A unit used to express distances on a genetic map. In genetic mapping, distances between markers are determined by measuring the rate of meoitic recombination between them, which increases proportionately with the distance separating them. A cM is defined as the length of an interval in which there is a 1% probability of recombination. On the average, 1 cM is roughly equivalent to 1 megabase (Mb) of DNA, although this can vary widely due to hot and cold spots of recombination." [http://www.ncbi.nlm.nih.gov/SCIENCE96/Glossary.html]
synonym: "cM" EXACT []
is_a: UO:0000001 ! length unit

[Term]
id: UO:0000327
name: centiRay
def: "A unit of genetic map distance defined corresponding to an interval in which there is a 1% probability of X-irradiation induced breakage. To be completely specified, the unit must be qualified by the radiation in dosage in rads (e.g. cR8000), because this determines the actual breakage probability." [http://www.ncbi.nlm.nih.gov/SCIENCE96/Glossary.html]
synonym: "cR" EXACT []
is_a: UO:0000001 ! length unit

[Term]
id: UO:0000328
name: kilo base pair
def: "A unit equal to one thousand base pairs." [UOC:GVG]
synonym: "kbp" EXACT []
synonym: "kilobasepair" EXACT []
is_a: UO:0000244 ! base pair

[Term]
id: UO:0000329
name: mega base pair
def: "A unit equal to one million base pairs" [UOC:GVG]
synonym: "Mb" EXACT []
synonym: "megabasepair" EXACT []
is_a: UO:0000244 ! base pair
intersection_of: UO:1000244 ! base pair based unit
intersection_of: has:prefix UO:0000293 ! mega
relationship: has:prefix UO:0000293 ! mega

[Term]
id: UO:0000330
name: giga base pair
def: "A unit equal to one billion base pairs." [UOC:GVG]
synonym: "Gb" EXACT []
synonym: "gigabasepair" EXACT []
is_a: UO:0000244 ! base pair
intersection_of: UO:1000244 ! base pair based unit
intersection_of: has:prefix UO:0000292 ! giga
relationship: has:prefix UO:0000292 ! giga

[Term]
id: UO:0000331
name: gigabyte
def: "An information unit which is equal to 1000000000 bytes." [UO:GVG]
synonym: "GB" EXACT []
is_a: UO:0000231 ! information unit

[Term]
id: UO:0000332
name: terabyte
def: "An information unit which is equal to 1000 gigabytes." [UO:GVG]
synonym: "TB" EXACT []
is_a: UO:0000231 ! information unit

[Term]
id: UO:0010001
name: square micrometer
def: "An area unit which is equal to an area enclosed by a square with sides each 1 micrometer long." [NIST:NIST]
synonym: "square micrometre" EXACT []
is_a: UO:1010001 ! square micrometer based unit

[Term]
id: UO:0010002
name: millisiemens
def: "An electrical conduction unit which is equal to one thousandth of a siemen or 10^[-3] siemens." [NIST:NIST]
synonym: "mS" RELATED []
is_a: UO:1000264 ! siemens based unit
intersection_of: UO:1000264 ! siemens based unit
intersection_of: has:prefix UO:0000297 ! milli
relationship: has:prefix UO:0000297 ! milli

[Term]
id: UO:0010003
name: micromole per litre
def: "A specific concentration unit which is equal to 1 micromole in a given volume of one thousandth of a cubic meter." [NIST:NIST]
is_a: UO:0000067 ! unit of molality

[Term]
id: UO:0010004
name: micromole per kilogram
def: "A specific concentration unit which is equal to 1 micromole of a given substance per kilogram of solvent." [UOB:LKSR]
is_a: UO:0000067 ! unit of molality

[Term]
id: UO:0010005
name: millimeters per day
def: "A speed/velocity unit which is equal to the speed of an object traveling 1 millimeter distance in one day." [UOB:LKSR]
synonym: "mm/day" EXACT []
is_a: UO:0000060 ! speed/velocity unit

[Term]
id: UO:0010006
name: ratio
def: "A dimensionless ratio unit which, given a pair of quantities a and b, for which b is a multiple of a, denotes b by giving the multiplier (coefficient) c for a to result in b." [UOB:LKSR]
is_a: UO:0000190 ! ratio unit

[Term]
id: UO:0010007
name: volt-second per square centimeter
def: "An electrical mobility unit which is equal to one volt second per square centimeter." [UOB:LKSR]
synonym: "volt-second per square centimetre" EXACT []
synonym: "Vs/cm^2" EXACT []
is_a: UO:0000262 ! electrical conduction unit

[Term]
id: UO:0010008
name: kilometer per hour
def: "A speed/velocity unit which is equal to the speed of an object traveling 1 kilometer distance in one hour." [NIST:NIST]
synonym: "kilometre per hour" EXACT []
synonym: "km/h" EXACT []
is_a: UO:0000060 ! speed/velocity unit

[Term]
id: UO:0010009
name: milli
def: "A mass unit which is equal to 1/12 the mass of 12C" [Wikipedia:Wikipedia]
synonym: "mDa" EXACT []
synonym: "milli unified atomic mass unit" EXACT []
synonym: "millidalton" EXACT []
synonym: "mmu" EXACT []
is_a: UO:0000002 ! mass unit

[Term]
id: UO:0010010
name: hectare
def: "An area unit which is equal to an area of 10,000 square meters. Equivalent to 2.471 acres." [Wikipedia:Wikipedia]
synonym: "HA" EXACT []
is_a: UO:1010010 ! hectare based unit

[Term]
id: UO:0010011
name: inch
def: "A length unit which is equal to 0.0254 metres." [Wikipedia:Wikpiedia]
synonym: "in" EXACT []
is_a: UO:0000045 ! base unit
is_a: UO:1010011 ! inch based unit

[Term]
id: UO:0010012
name: thou
def: "A length unit which is equal to 0.0254 millimetres." [Wikipedia:Wikpiedia]
synonym: "mil" EXACT []
synonym: "th" EXACT []
is_a: UO:0000045 ! base unit
is_a: UO:1010012 ! thou based unit

[Term]
id: UO:0010013
name: foot
def: "A length unit which is equal to 0.3048 metres, or 12 inches." [Wikipedia:Wikpiedia]
synonym: "ft" EXACT []
is_a: UO:0000045 ! base unit
is_a: UO:1010013 ! foot based unit

[Term]
id: UO:0010014
name: yard
def: "A length unit which is equal to 0.9144 metres, or 3 feet." [Wikipedia:Wikpiedia]
synonym: "yd" EXACT []
is_a: UO:0000045 ! base unit
is_a: UO:1010014 ! yard based unit

[Term]
id: UO:0010015
name: chain
def: "A length unit which is equal to 20.1168 metres, 66 feet, or 22 yards." [Wikipedia:Wikpiedia]
synonym: "ch" EXACT []
is_a: UO:0000045 ! base unit
is_a: UO:1010015 ! chain based unit

[Term]
id: UO:0010016
name: furlong
def: "A length unit which is equal to 20,116.8 metres, 660 feet, or 10 chains." [Wikipedia:Wikpiedia]
synonym: "fur" EXACT []
is_a: UO:0000045 ! base unit
is_a: UO:1010016 ! furlong based unit

[Term]
id: UO:0010017
name: mile
def: "A length unit which is equal to 1,609.344 metres, or 8 furlongs." [Wikipedia:Wikpiedia]
synonym: "mi" EXACT []
is_a: UO:0000045 ! base unit
is_a: UO:1010017 ! mile based unit

[Term]
id: UO:0010018
name: league
def: "A length unit which is equal to 3 miles, or 4,828.032 metres" [Wikipedia:Wikpiedia]
synonym: "lea" EXACT []
is_a: UO:0000045 ! base unit
is_a: UO:1010018 ! league based unit

[Term]
id: UO:0010019
name: maritime length unit
def: "A maritime length unit is one used primarily at sea." [Wikipedia:Wikpiedia]
is_a: UO:1010019 ! maritime length unit based unit

[Term]
id: UO:0010020
name: fathom
def: "A maritime length unit which is equal to 6.08 feet, or 1.853184 metres" [Wikipedia:Wikpiedia]
synonym: "ftm" EXACT []
is_a: UO:1010020 ! fathom based unit

[Term]
id: UO:0010021
name: cable
def: "A maritime length unit which is equal to 608 feet, 100 fathoms, or 185.3184 metres" [Wikipedia:Wikpiedia]
is_a: UO:1010021 ! cable based unit

[Term]
id: UO:0010022
name: nautical mile
def: "A maritime length unit which is equal to 6,080 feet, 10 cables, or 1,853.184 metres" [Wikipedia:Wikpiedia]
is_a: UO:1010022 ! nautical mile based unit

[Term]
id: UO:0010023
name: perch
def: "An area unit which is equal to an area of 25.292,852,64 square meters, or 1 square rod." [Wikipedia:Wikipedia]
is_a: UO:1010023 ! perch based unit

[Term]
id: UO:0010024
name: rood
def: "An area unit which is equivalent to 1 furlong x 1 rod. This is equal to an area of 1,011.714,1056 square meters, or 40 square rods." [Wikipedia:Wikipedia]
is_a: UO:1010024 ! rood based unit

[Term]
id: UO:0010025
name: acre
def: "An area unit which is equivalent to 1 furlong x 1 chain. This is equal to an area of 4,046.856,4224 square meters, or 43,500 square feet." [Wikipedia:Wikipedia]
is_a: UO:1010025 ! acre based unit

[Term]
id: UO:0010026
name: fluid ounce
def: "An imperial volume unit which is equivalent to 28.413,0625 millilitres." [Wikipedia:Wikipedia]
synonym: "fl oz" EXACT []
is_a: UO:1010026 ! fluid ounce based unit

[Term]
id: UO:0010027
name: gill
def: "An imperial volume unit which is equivalent to 142.065,3125 millilitres." [Wikipedia:Wikipedia]
synonym: "gi" EXACT []
is_a: UO:1010027 ! gill based unit

[Term]
id: UO:0010028
name: pint
def: "An imperial volume unit which is equivalent to 568.261,25 millilitres." [Wikipedia:Wikipedia]
synonym: "pt" EXACT []
is_a: UO:1010028 ! pint based unit

[Term]
id: UO:0010029
name: quart
def: "An imperial volume unit which is equivalent to 1,136.5225 millilitres, or two pints." [Wikipedia:Wikipedia]
synonym: "qt" EXACT []
is_a: UO:1010029 ! quart based unit

[Term]
id: UO:0010030
name: gallon
def: "An imperial volume unit which is equivalent to 4,546.09 millilitres, or 8 pints." [Wikipedia:Wikipedia]
synonym: "gal" EXACT []
is_a: UO:1010030 ! gallon based unit

[Term]
id: UO:0010031
name: grain
def: "An imperial mass unit which is equivalent to 64.798,91 milligrams." [Wikipedia:Wikipedia]
synonym: "gr" EXACT []
is_a: UO:1010031 ! grain based unit

[Term]
id: UO:0010032
name: drachm
def: "An imperial mass unit which is equivalent to 1.771,845,195,3125 grams, or 1/256 of 1 pound." [Wikipedia:Wikipedia]
synonym: "dr" EXACT []
is_a: UO:1010032 ! drachm based unit

[Term]
id: UO:0010033
name: ounce
def: "An imperial mass unit which is equivalent to 28.349,523,125 grams, or 1/16 of 1 pound." [Wikipedia:Wikipedia]
synonym: "oz" EXACT []
is_a: UO:1010033 ! ounce based unit

[Term]
id: UO:0010034
name: pound
def: "An imperial mass unit which is equivalent to 453.592,37 grams." [Wikipedia:Wikipedia]
synonym: "lb" EXACT []
is_a: UO:1010034 ! pound based unit

[Term]
id: UO:0010035
name: stone
def: "An imperial mass unit which is equivalent to 6,350.293,18 grams, or 14 pounds." [Wikipedia:Wikipedia]
synonym: "st" EXACT []
is_a: UO:1010035 ! stone based unit

[Term]
id: UO:0010036
name: quarter
def: "An imperial mass unit which is equivalent to 12.700,586,36 kilograms, or 28 pounds." [Wikipedia:Wikipedia]
synonym: "qr" EXACT []
synonym: "qtr" EXACT []
is_a: UO:1010036 ! quarter based unit

[Term]
id: UO:0010037
name: hundredweight
def: "An imperial mass unit which is equivalent to 50.802,345,44 kilograms, 112 pounds, or 8 stone." [Wikipedia:Wikipedia]
synonym: "cwt" EXACT []
is_a: UO:1010037 ! hundredweight based unit

[Term]
id: UO:0010038
name: ton
def: "An imperial mass unit which is equivalent to 1,016.046,9088 kilograms, or 2,240 pounds." [Wikipedia:Wikipedia]
synonym: "t" EXACT []
is_a: UO:1010038 ! ton based unit

[Term]
id: UO:0010039
name: slug
def: "An imperial gravitational unit which is equivalent to a mass that accelerates by 1ft/sÂ² when a force of one pound (lbf) is exerted on it." [Wikipedia:Wikipedia]
is_a: UO:1010039 ! slug based unit

[Term]
id: UO:0010040
name: teaspoon
def: "A metric teaspoon is a unit of measurement of volume widely used in cooking recipes and pharmaceutic prescriptions. It equals a 5mL volume." [Wikipedia:Teaspoon]
synonym: "metric teaspoon" EXACT []
synonym: "tsp" EXACT []
is_a: UO:1010040 ! teaspoon based unit

[Term]
id: UO:0010041
name: united states customary teaspoon
def: "A United States customary units teaspoon is a unit of measurement of volume widely used in cooking recipes and pharmaceutic prescriptions in America. It equals a 4.93 mL volume." [Wikipedia:United_States_customary_units#Cooking_measures]
synonym: "us customary teaspoon" EXACT []
is_a: UO:0000095 ! volume unit

[Term]
id: UO:0010042
name: tablespoon
def: "A metric tablespoon is a unit of measurement of volume widely used in cooking recipes and pharmaceutic prescriptions. It equals a 15mL volume." [Wikipedia:Tablespoon]
synonym: "metric tablespoon" EXACT []
synonym: "tbsp" EXACT []
is_a: UO:0000095 ! volume unit

[Term]
id: UO:0010043
name: australian metric tablespoon
def: "An Australian metric tablespoon is a unit of measurement of volume used in Australia for cooking recipes and pharmaceutic prescriptions. It equals a 20mL volume." [Wikipedia:Tablespoon]
is_a: UO:0000095 ! volume unit

[Term]
id: UO:0010044
name: united states customary tablespoon
def: "A United States customary units tablespoon is a unit of measurement of volume widely used in cooking recipes and pharmaceutic prescriptions in America. It equals a 14.79 mL volume." [Wikipedia:United_States_customary_units#Cooking_measures]
synonym: "us customary tablespoon" EXACT []
is_a: UO:0000095 ! volume unit

[Term]
id: UO:0010045
name: metric cup
def: "A metric cup is a unit of measurement of volume widely used in cooking recipes and pharmaceutic prescriptions. It equals a 250mL volume." [Wikipedia:Cooking_weights_and_measures]
synonym: "C" EXACT []
is_a: UO:0000095 ! volume unit

[Term]
id: UO:0010046
name: united states customary cup
def: "A United States customary units cup is a unit of measurement of volume widely used in cooking recipes and pharmaceutic prescriptions in America. It equals a 236.59 mL volume." [Wikipedia:United_States_customary_units#Cooking_measures]
synonym: "us customary cup" EXACT []
is_a: UO:0000095 ! volume unit

[Term]
id: UO:0010047
name: united states fda cup
def: "A United States FDA cup is a unit of measurement of volume used by the US Federal Department of Agriculture as a nutritional serving measure. It equals a 240 mL volume." [Wikipedia:United_States_customary_units#Cooking_measures]
synonym: "us fda cup" EXACT []
is_a: UO:0000095 ! volume unit

[Term]
id: UO:0010048
name: micromole
def: "DEPRECATED: Duplicate of http://purl.obolibrary.org/obo/UO_0000039. A substance unit which is equal to one millionth of a mole." [UOB:LTS]
is_a: UO:0000006 ! substance unit
is_obsolete: true

[Term]
id: UO:0010049
name: gram per square meter
def: "An area density unit which is equal to the mass of an object in grams divided by the surface area in meters squared." [NIST:NIST]
synonym: "g/m^[2]" EXACT []
synonym: "gram per square metre" EXACT []
is_a: UO:1010049 ! gram per square meter based unit

[Term]
id: UO:0010050
name: nanogram per microliter
def: "A mass unit density which is equal to mass of an object in nanograms divided by the volume in microliters." [UOB:LTS]
synonym: "nanogram per microlitre" EXACT []
synonym: "ng/ul" EXACT []
is_a: UO:0000052 ! mass density unit

[Term]
id: UO:0010051
name: large calorie
def: "A unit of energy widely used in nutrition, equivalent to the amount of heat needed to cause one kilogram of water to rise in temperature by one degree Celsius." [Wikipedia:Wikipedia]
synonym: "big calorie" EXACT []
synonym: "cal" EXACT []
synonym: "calorie" EXACT []
synonym: "food calorie" EXACT []
synonym: "kcal" EXACT []
synonym: "kilocalorie" EXACT []
is_a: UO:1010051 ! large calorie based unit

[Term]
id: UO:0010052
name: pounds per square inch
def: "A pressure unit which is equal to 6894.757 pascal." [Wikipedia:Wikipedia]
synonym: "lbf/in^[2]" EXACT []
synonym: "psi" EXACT []
is_a: UO:0000109 ! pressure unit

[Term]
id: UO:0010053
name: micrograms per wheaton bottle
def: "A unit of mass concentration defined as the number of micrograms of a substance per 250 ml Wheaton bottle." [UOB:LTS]
synonym: "micrograms per bottle" EXACT []
is_a: UO:0000052 ! mass density unit

[Term]
id: UO:0010054
name: picoampere
def: "An electric current unit current which is equal to one trillionth of an ampere or 10^[-12] A." [UOB:LTS]
synonym: "pA" EXACT []
is_a: UO:1000011 ! ampere based unit
intersection_of: UO:1000011 ! ampere based unit
intersection_of: has:prefix UO:0000302 ! pico
relationship: has:prefix UO:0000302 ! pico

[Term]
id: UO:0010055
name: centigray
def: "An absorbed dose unit which is equal to 0.01 gray (Gy)" [NIST:NIST]
synonym: "cGy" EXACT []
is_a: UO:1000134 ! gray based unit
intersection_of: UO:1000134 ! gray based unit
intersection_of: has:prefix UO:0000298 ! centi
relationship: has:prefix UO:0000298 ! centi

[Term]
id: UO:0010056
name: gigaelectronvolt
def: "A unit of energy that is equal to one thousand million electronvolts." []
synonym: "GeV" EXACT []
is_a: UO:1000266 ! electronvolt based unit
intersection_of: UO:1000266 ! electronvolt based unit
intersection_of: has:prefix UO:0000292 ! giga
relationship: has:prefix UO:0000292 ! giga

[Term]
id: UO:0010057
name: gigaelectronvolt per nucleon
def: "Derived unit which is equal to the total kinetic energy of an atomic nucleus in GeV divided by the number of nucleons in the nucleus" []
synonym: "GeV/nucleon" EXACT []
is_a: UO:0000111 ! energy unit

[Term]
id: UO:0010058
name: megaelectronvolt per nucleon
def: "Derived unit which is equal to the total kinetic energy of an atomic nucleus in MeV divided by the number of nucleons in the nucleus" []
synonym: "MeV/nucleon" EXACT []
is_a: UO:0000111 ! energy unit

[Term]
id: UO:0010059
name: kiloelectronvolt per micron
def: "A derived unit equal to the energy deposited by ionizing radiation per micron of path length in matter" []
synonym: "keV/micron" EXACT []
is_a: UO:0000111 ! energy unit

[Term]
id: UO:0010060
name: gray per minute
def: "A derived absorbed dose unit which is equal to one gray absorbed per minute." [NIST:NIST]
synonym: "Gy/min" EXACT []
is_a: UO:1010060 ! gray per minute based unit

[Term]
id: UO:0010061
name: centigray per minute
def: "A derived absorbed dose unit which is equal to one centigray absorbed per minute." [NIST:NIST]
synonym: "cGy/min" EXACT []
is_a: UO:1010060 ! gray per minute based unit
intersection_of: UO:1010060 ! gray per minute based unit
intersection_of: has:prefix UO:0000298 ! centi
relationship: has:prefix UO:0000298 ! centi

[Term]
id: UO:0010062
name: milligray per minute
def: "A derived absorbed dose unit which is equal to one milligray absorbed per minute." [NIST:NIST]
synonym: "mGy/day" EXACT []
is_a: UO:1010060 ! gray per minute based unit
intersection_of: UO:1010060 ! gray per minute based unit
intersection_of: has:prefix UO:0000297 ! milli
relationship: has:prefix UO:0000297 ! milli

[Term]
id: UO:0010063
name: milligray per day
def: "A derived absorbed dose unit which is equal to one milligray absorbed per day." [NIST:NIST]
synonym: "mGy/min" EXACT []
is_a: UO:0000129 ! absorbed dose unit

[Term]
id: UO:0010064
name: milligray per hour
def: "A derived absorbed dose unit which is equal to one milligray absorbed per hour." [NIST:NIST]
synonym: "mGy/h" EXACT []
is_a: UO:0000129 ! absorbed dose unit

[Term]
id: UO:0010065
name: milligray per second
def: "A derived absorbed dose unit which is equal to one milligray absorbed per second." [NIST:NIST]
synonym: "mGy/s" EXACT []
is_a: UO:0000129 ! absorbed dose unit

[Term]
id: UO:0010066
name: kilometer
def: "A length unit which is equal to one thousand meters." [UOB:LKSR]
synonym: "kilometre" EXACT []
synonym: "km" EXACT []
is_a: UO:1000008 ! meter based unit
intersection_of: UO:1000008 ! meter based unit
intersection_of: has:prefix UO:0000294 ! kilo
relationship: has:prefix UO:0000294 ! kilo

[Term]
id: UO:0010067
name: milligram per deciliter
def: "A mass unit density which is equal to mass of an object in milligrams divided by the volume in deciliters." [UOB:LKSR]
synonym: "mg/dl" EXACT []
synonym: "milligram per decilitre" EXACT []
is_a: UO:1000208 ! gram per deciliter based unit
intersection_of: UO:1000208 ! gram per deciliter based unit
intersection_of: has:prefix UO:0000297 ! milli
relationship: has:prefix UO:0000297 ! milli

[Term]
id: UO:0010068
name: microgram per deciliter
def: "A mass unit density which is equal to mass of an object in micrograms divided by the volume in deciliters." [UOB:LKSR]
synonym: "microgram per decilitre" EXACT []
synonym: "ug/dl" EXACT []
is_a: UO:1000208 ! gram per deciliter based unit
intersection_of: UO:1000208 ! gram per deciliter based unit
intersection_of: has:prefix UO:0000299 ! micro
relationship: has:prefix UO:0000299 ! micro

[Term]
id: UO:0010069
name: bar
def: "A pressure unit which is equal to 100,000 pascal or the pressure or stress on a surface caused by a force of 100,000 newtons spread over a surface of 1 m^[2]." [NIST:NIST]
is_a: UO:1000110 ! pascal based unit

[Term]
id: UO:0010070
name: picogram per milliliter
def: "A gram per milliliter unit which is equal to one picogram per one milliliter." []
synonym: "pg/mL" EXACT []
is_a: UO:1000173 ! gram per milliliter based unit

[Term]
id: UO:0010071
name: microgram per square centimeter
def: "An area density unit which is equal to the mass of an object in micrograms divided by the surface area in square centimeters." []
synonym: "mcg/cm2" EXACT []
synonym: "Âµg/cmÂ²" EXACT []
is_a: UO:0000054 ! area density unit

[Term]
id: UO:0010072
name: microgram per microliter
def: "A mass unit density which is equal to mass of an object in nanograms divided by the volume in microliters." [UOB:LTS]
synonym: "mcg/mcL" EXACT []
synonym: "ug/uL" EXACT []
synonym: "Âµg/ÂµL" EXACT []
is_a: UO:0000052 ! mass density unit

[Term]
id: UO:0010073
name: cell count
def: "A count unit that denotes a count of cells." []
is_a: UO:0000189 ! count unit

[Term]
id: UO:0010074
name: heartbeats per minute
def: "A rate unit which represents a measurement of the number of an organism's heartbeats per one minute." []
synonym: "BPM" EXACT []
is_a: UO:0000280 ! rate unit

[Term]
id: UO:0010075
name: multiplicity of infection
def: "A ratio unit which denotes the quantity of infectious agents to infection targets." []
synonym: "MOI" EXACT []
is_a: UO:0000190 ! ratio unit

[Term]
id: UO:0010076
name: breaths per minute
def: "A rate unit which represents a measurement of the number of breaths taken by an organism per one minute." []
synonym: "br/min" EXACT []
synonym: "brpm" EXACT []
is_a: UO:0000280 ! rate unit

[Term]
id: UO:0010077
name: PCR quantification cycle
def: "A count unit of how many Polymerase Chain Reaction (PCR) cycles it took toÂ detect a real signalÂ from a sample. Equivalent to the PCR cycle number at which a sample's reaction curve intersects the threshold line." []
synonym: "Ct" EXACT []
is_a: UO:0000189 ! count unit

[Term]
id: UO:0010080
name: titer
def: "A concentration unit which denotes the minimum amount of a substance in a solution that still yields a positive reading, as determined by serial dilution." []
is_a: UO:0000051 ! concentration unit

[Term]
id: UO:1000008
name: meter based unit
is_a: UO:0000001 ! length unit

[Term]
id: UO:1000010
name: second based unit
is_a: UO:0000003 ! time unit

[Term]
id: UO:1000011
name: ampere based unit
is_a: UO:0000004 ! electric current unit

[Term]
id: UO:1000012
name: kelvin based unit
is_a: UO:0000005 ! temperature unit

[Term]
id: UO:1000013
name: mole based unit
is_a: UO:0000006 ! substance unit

[Term]
id: UO:1000014
name: candela based unit
is_a: UO:0000007 ! luminous intensity unit

[Term]
id: UO:1000019
name: angstrom based unit
is_a: UO:0000001 ! length unit

[Term]
id: UO:1000021
name: gram based unit
is_a: UO:0000002 ! mass unit

[Term]
id: UO:1000027
name: degree Celsius based unit
is_a: UO:0000005 ! temperature unit

[Term]
id: UO:1000031
name: minute based unit
is_a: UO:0000003 ! time unit

[Term]
id: UO:1000032
name: hour based unit
is_a: UO:0000003 ! time unit

[Term]
id: UO:1000033
name: day based unit
is_a: UO:0000003 ! time unit

[Term]
id: UO:1000034
name: week based unit
is_a: UO:0000003 ! time unit

[Term]
id: UO:1000035
name: month based unit
is_a: UO:0000003 ! time unit

[Term]
id: UO:1000036
name: year based unit
is_a: UO:0000003 ! time unit

[Term]
id: UO:1000062
name: molar based unit
is_a: UO:0000061 ! unit of molarity

[Term]
id: UO:1000068
name: molal based unit
is_a: UO:0000067 ! unit of molality

[Term]
id: UO:1000075
name: normal based unit
is_a: UO:0000074 ! unit of normality

[Term]
id: UO:1000076
name: mole fraction based unit
is_a: UO:0000051 ! concentration unit
is_a: UO:0000191 ! fraction

[Term]
id: UO:1000077
name: meter per second per second based unit
is_a: UO:0000048 ! acceleration unit

[Term]
id: UO:1000078
name: radian per second per second based unit
is_a: UO:0000050 ! angular acceleration unit

[Term]
id: UO:1000079
name: radian per second based unit
is_a: UO:0000049 ! angular velocity unit

[Term]
id: UO:1000080
name: square meter based unit
is_a: UO:0000047 ! area unit

[Term]
id: UO:1000081
name: square centimeter based unit
is_a: UO:0000047 ! area unit

[Term]
id: UO:1000082
name: square millimeter based unit
is_a: UO:0000047 ! area unit

[Term]
id: UO:1000084
name: gram per cubic centimeter based unit
is_a: UO:0000052 ! mass density unit

[Term]
id: UO:1000085
name: candela per square meter based unit
is_a: UO:0000053 ! luminance unit

[Term]
id: UO:1000088
name: gram per mole based unit
is_a: UO:0000055 ! molar mass unit

[Term]
id: UO:1000089
name: cubic meter per mole based unit
is_a: UO:0000056 ! molar volume unit

[Term]
id: UO:1000090
name: cubic centimeter per mole based unit
is_a: UO:0000056 ! molar volume unit

[Term]
id: UO:1000092
name: turns per second based unit
is_a: UO:0000058 ! rotational frequency unit

[Term]
id: UO:1000093
name: cubic meter per kilogram based unit
is_a: UO:0000059 ! specific volume unit

[Term]
id: UO:1000094
name: meter per second based unit
is_a: UO:0000060 ! speed/velocity unit

[Term]
id: UO:1000096
name: cubic meter based unit
is_a: UO:0000095 ! volume unit

[Term]
id: UO:1000097
name: cubic centimeter based unit
is_a: UO:0000095 ! volume unit

[Term]
id: UO:1000099
name: liter based unit
is_a: UO:0000095 ! volume unit

[Term]
id: UO:1000100
name: cubic decimeter based unit
is_a: UO:0000095 ! volume unit

[Term]
id: UO:1000106
name: hertz based unit
is_a: UO:0000105 ! frequency unit

[Term]
id: UO:1000108
name: newton based unit
is_a: UO:0000107 ! force unit

[Term]
id: UO:1000110
name: pascal based unit
is_a: UO:0000109 ! pressure unit

[Term]
id: UO:1000112
name: joule based unit
is_a: UO:0000111 ! energy unit

[Term]
id: UO:1000114
name: watt based unit
is_a: UO:0000113 ! power unit

[Term]
id: UO:1000116
name: lux based unit
is_a: UO:0000115 ! illuminance unit

[Term]
id: UO:1000118
name: lumen based unit
is_a: UO:0000117 ! luminous flux unit

[Term]
id: UO:1000120
name: katal based unit
is_a: UO:0000119 ! catalytic activity unit

[Term]
id: UO:1000123
name: radian based unit
is_a: UO:0000122 ! plane angle unit

[Term]
id: UO:1000125
name: steradian based unit
is_a: UO:0000124 ! solid angle unit

[Term]
id: UO:1000132
name: becquerel based unit
is_a: UO:0000128 ! activity (of a radionuclide) unit

[Term]
id: UO:1000133
name: curie based unit
is_a: UO:0000128 ! activity (of a radionuclide) unit

[Term]
id: UO:1000134
name: gray based unit
is_a: UO:0000129 ! absorbed dose unit

[Term]
id: UO:1000135
name: rad based unit
is_a: UO:0000129 ! absorbed dose unit

[Term]
id: UO:1000136
name: roentgen based unit
is_a: UO:0000131 ! exposure unit

[Term]
id: UO:1000137
name: sievert based unit
is_a: UO:0000130 ! dose equivalent unit

[Term]
id: UO:1000140
name: Roentgen equivalent man based unit
is_a: UO:0000130 ! dose equivalent unit

[Term]
id: UO:1000147
name: disintegrations per minute based unit
is_a: UO:0000128 ! activity (of a radionuclide) unit

[Term]
id: UO:1000148
name: counts per minute based unit
is_a: UO:0000128 ! activity (of a radionuclide) unit

[Term]
id: UO:1000151
name: century based unit
is_a: UO:0000003 ! time unit

[Term]
id: UO:1000152
name: half life based unit
is_a: UO:0000003 ! time unit

[Term]
id: UO:1000153
name: foot candle based unit
is_a: UO:0000115 ! illuminance unit

[Term]
id: UO:1000155
name: watt per square meter based unit
is_a: UO:0000154 ! irradiance unit

[Term]
id: UO:1000156
name: einstein per square meter per second based unit
is_a: UO:0000154 ! irradiance unit

[Term]
id: UO:1000158
name: watt per steradian per square meter based unit
is_a: UO:0000161 ! radiance unit

[Term]
id: UO:1000162
name: watt per steradian based unit
is_a: UO:0000159 ! radiant intensity unit

[Term]
id: UO:1000163
name: mass percentage based unit
is_a: UO:0000051 ! concentration unit
is_a: UO:0000187 ! percent

[Term]
id: UO:1000164
name: mass volume percentage based unit
is_a: UO:0000051 ! concentration unit
is_a: UO:0000187 ! percent

[Term]
id: UO:1000165
name: volume percentage based unit
is_a: UO:0000187 ! percent
is_a: UO:0000205 ! volume per unit volume

[Term]
id: UO:1000167
name: parts per hundred based unit
is_a: UO:0000166 ! parts per notation unit

[Term]
id: UO:1000168
name: parts per thousand based unit
is_a: UO:0000166 ! parts per notation unit

[Term]
id: UO:1000169
name: parts per million based unit
is_a: UO:0000166 ! parts per notation unit

[Term]
id: UO:1000170
name: parts per billion based unit
is_a: UO:0000166 ! parts per notation unit

[Term]
id: UO:1000171
name: parts per trillion based unit
is_a: UO:0000166 ! parts per notation unit

[Term]
id: UO:1000172
name: parts per quadrillion based unit
is_a: UO:0000166 ! parts per notation unit

[Term]
id: UO:1000173
name: gram per milliliter based unit
is_a: UO:0000052 ! mass density unit

[Term]
id: UO:1000175
name: gram per liter based unit
is_a: UO:0000052 ! mass density unit

[Term]
id: UO:1000178
name: unit per milliliter based unit
is_a: UO:0000177 ! unit per volume unit

[Term]
id: UO:1000179
name: unit per liter based unit
is_a: UO:0000177 ! unit per volume unit

[Term]
id: UO:1000180
name: mass per unit volume based unit
is_a: UO:0000051 ! concentration unit

[Term]
id: UO:1000181
name: enzyme unit based unit
is_a: UO:0000119 ! catalytic activity unit

[Term]
id: UO:1000185
name: degree based unit
is_a: UO:0000122 ! plane angle unit

[Term]
id: UO:1000188
name: pi based unit
is_a: UO:0000186 ! dimensionless unit

[Term]
id: UO:1000192
name: molecule count based unit
is_a: UO:0000189 ! count unit

[Term]
id: UO:1000193
name: purity percentage based unit
is_a: UO:0000187 ! percent

[Term]
id: UO:1000194
name: confluence percentage based unit
is_a: UO:0000187 ! percent

[Term]
id: UO:1000195
name: degree Fahrenheit based unit
is_a: UO:0000005 ! temperature unit

[Term]
id: UO:1000196
name: pH based unit
is_a: UO:0000051 ! concentration unit
is_a: UO:0000186 ! dimensionless unit

[Term]
id: UO:1000197
name: liter per kilogram based unit
is_a: UO:0000059 ! specific volume unit

[Term]
id: UO:1000201
name: cells per milliliter based unit
is_a: UO:0000200 ! cell concentration unit

[Term]
id: UO:1000203
name: katal per cubic meter based unit
is_a: UO:0000202 ! catalytic (activity) concentration unit

[Term]
id: UO:1000204
name: katal per liter based unit
is_a: UO:0000202 ! catalytic (activity) concentration unit

[Term]
id: UO:1000208
name: gram per deciliter based unit
is_a: UO:0000052 ! mass density unit

[Term]
id: UO:1000210
name: colony forming unit based unit
is_a: UO:0000189 ! count unit

[Term]
id: UO:1000211
name: plaque forming unit based unit
is_a: UO:0000189 ! count unit

[Term]
id: UO:1000213
name: colony forming unit per milliliter based unit
is_a: UO:0000212 ! colony forming unit per volume

[Term]
id: UO:1000215
name: plaque forming unit per milliliter based unit
is_a: UO:0000214 ! plaque forming unit per volume

[Term]
id: UO:1000216
name: disintegrations per second based unit
is_a: UO:0000128 ! activity (of a radionuclide) unit

[Term]
id: UO:1000218
name: volt based unit
is_a: UO:0000217 ! electric potential difference unit

[Term]
id: UO:1000220
name: coulomb based unit
is_a: UO:0000219 ! electric charge

[Term]
id: UO:1000221
name: dalton based unit
is_a: UO:0000002 ! mass unit

[Term]
id: UO:1000223
name: watt-hour based unit
is_a: UO:0000111 ! energy unit

[Term]
id: UO:1000226
name: weber based unit
is_a: UO:0000225 ! magnetic flux unit

[Term]
id: UO:1000228
name: tesla based unit
is_a: UO:0000227 ! magnetic flux density unit

[Term]
id: UO:1000229
name: volt-hour based unit
is_a: UO:0000225 ! magnetic flux unit

[Term]
id: UO:1000232
name: bit based unit
is_a: UO:0000231 ! information unit

[Term]
id: UO:1000233
name: byte based unit
is_a: UO:0000231 ! information unit

[Term]
id: UO:1000237
name: chroma sampling unit based unit
is_a: UO:0000236 ! image resolution unit

[Term]
id: UO:1000238
name: dynamic range unit based unit
is_a: UO:0000236 ! image resolution unit

[Term]
id: UO:1000240
name: dots per inch based unit
is_a: UO:0000239 ! spatial resolution unit

[Term]
id: UO:1000242
name: pixels per inch based unit
is_a: UO:0000239 ! spatial resolution unit

[Term]
id: UO:1000243
name: pixels per millimeter based unit
is_a: UO:0000239 ! spatial resolution unit

[Term]
id: UO:1000244
name: base pair based unit
is_a: UO:0000189 ! count unit

[Term]
id: UO:1000245
name: kibibyte based unit
is_a: UO:0000231 ! information unit

[Term]
id: UO:1000246
name: mebibyte based unit
is_a: UO:0000231 ! information unit

[Term]
id: UO:1000254
name: newton per meter based unit
is_a: UO:0000253 ! surface tension unit

[Term]
id: UO:1000255
name: dyne per cm based unit
is_a: UO:0000253 ! surface tension unit

[Term]
id: UO:1000257
name: pascal second based unit
is_a: UO:0000256 ! viscosity unit

[Term]
id: UO:1000258
name: poise based unit
is_a: UO:0000256 ! viscosity unit

[Term]
id: UO:1000260
name: effective dose unit based unit
is_a: UO:0000127 ! radiation unit

[Term]
id: UO:1000264
name: siemens based unit
is_a: UO:0000262 ! electrical conduction unit

[Term]
id: UO:1000265
name: watt per meter kelvin based unit
is_a: UO:0000263 ! heat conduction unit

[Term]
id: UO:1000266
name: electronvolt based unit
is_a: UO:0000111 ! energy unit

[Term]
id: UO:1000268
name: volt per meter based unit
is_a: UO:0000267 ! electric field strength unit

[Term]
id: UO:1000269
name: absorbance unit based unit
is_a: UO:0000186 ! dimensionless unit

[Term]
id: UO:1000281
name: count per nanomolar second based unit
is_a: UO:0000280 ! rate unit

[Term]
id: UO:1000282
name: count per molar second based unit
is_a: UO:0000280 ! rate unit

[Term]
id: UO:1000284
name: count per nanomolar based unit
is_a: UO:0000280 ! rate unit

[Term]
id: UO:1000285
name: count per molar based unit
is_a: UO:0000280 ! rate unit

[Term]
id: UO:1000310
name: dosage unit based unit
is_a: UO:0000051 ! concentration unit

[Term]
id: UO:1000312
name: relative light unit based unit
is_a: UO:0000157 ! light unit

[Term]
id: UO:1000313
name: relative luminescence unit based unit
is_a: UO:0000312 ! relative light unit

[Term]
id: UO:1000314
name: relative fluorescence unit based unit
is_a: UO:0000312 ! relative light unit

[Term]
id: UO:1010001
name: square micrometer based unit
is_a: UO:0000047 ! area unit

[Term]
id: UO:1010010
name: hectare based unit
is_a: UO:0000047 ! area unit

[Term]
id: UO:1010011
name: inch based unit
is_a: UO:0000001 ! length unit

[Term]
id: UO:1010012
name: thou based unit
is_a: UO:0000001 ! length unit

[Term]
id: UO:1010013
name: foot based unit
is_a: UO:0000001 ! length unit

[Term]
id: UO:1010014
name: yard based unit
is_a: UO:0000001 ! length unit

[Term]
id: UO:1010015
name: chain based unit
is_a: UO:0000001 ! length unit

[Term]
id: UO:1010016
name: furlong based unit
is_a: UO:0000001 ! length unit

[Term]
id: UO:1010017
name: mile based unit
is_a: UO:0000001 ! length unit

[Term]
id: UO:1010018
name: league based unit
is_a: UO:0000001 ! length unit

[Term]
id: UO:1010019
name: maritime length unit based unit
is_a: UO:0000001 ! length unit

[Term]
id: UO:1010020
name: fathom based unit
is_a: UO:0010019 ! maritime length unit

[Term]
id: UO:1010021
name: cable based unit
is_a: UO:0010019 ! maritime length unit

[Term]
id: UO:1010022
name: nautical mile based unit
is_a: UO:0010019 ! maritime length unit

[Term]
id: UO:1010023
name: perch based unit
is_a: UO:0000047 ! area unit

[Term]
id: UO:1010024
name: rood based unit
is_a: UO:0000047 ! area unit

[Term]
id: UO:1010025
name: acre based unit
is_a: UO:0000047 ! area unit

[Term]
id: UO:1010026
name: fluid ounce based unit
is_a: UO:0000095 ! volume unit

[Term]
id: UO:1010027
name: gill based unit
is_a: UO:0000095 ! volume unit

[Term]
id: UO:1010028
name: pint based unit
is_a: UO:0000095 ! volume unit

[Term]
id: UO:1010029
name: quart based unit
is_a: UO:0000095 ! volume unit

[Term]
id: UO:1010030
name: gallon based unit
is_a: UO:0000095 ! volume unit

[Term]
id: UO:1010031
name: grain based unit
is_a: UO:0000002 ! mass unit

[Term]
id: UO:1010032
name: drachm based unit
is_a: UO:0000002 ! mass unit

[Term]
id: UO:1010033
name: ounce based unit
is_a: UO:0000002 ! mass unit

[Term]
id: UO:1010034
name: pound based unit
is_a: UO:0000002 ! mass unit

[Term]
id: UO:1010035
name: stone based unit
is_a: UO:0000002 ! mass unit

[Term]
id: UO:1010036
name: quarter based unit
is_a: UO:0000002 ! mass unit

[Term]
id: UO:1010037
name: hundredweight based unit
is_a: UO:0000002 ! mass unit

[Term]
id: UO:1010038
name: ton based unit
is_a: UO:0000002 ! mass unit

[Term]
id: UO:1010039
name: slug based unit
is_a: UO:0000111 ! energy unit

[Term]
id: UO:1010040
name: teaspoon based unit
is_a: UO:0000095 ! volume unit

[Term]
id: UO:1010049
name: gram per square meter based unit
is_a: UO:0000054 ! area density unit

[Term]
id: UO:1010051
name: large calorie based unit
is_a: UO:0000111 ! energy unit

[Term]
id: UO:1010060
name: gray per minute based unit
is_a: UO:0000129 ! absorbed dose unit

